Added "witness" clauses to newtype and subset-type declarations. Resolution and verification are done, but the compilation support for these is still missing. Fixed resolution bug that occurred when type declarations had cyclic dependencies.

Source/Dafny/Parser.cs
@@ -78,7 +78,7 @@ public class Parser {
 	public const int _notIn = 62;
 	public const int _ellipsis = 63;
 	public const int _reveal = 64;
-	public const int maxT = 149;
+	public const int maxT = 150;
 
   const bool _T = true;
   const bool _x = false;
@@ -800,12 +800,12 @@ int StringToInt(string s, int defaultValue, string errString) {
 			module.TopLevelDecls.Add(td); 
 			break;
 		}
-		case 88: {
+		case 89: {
 			OtherTypeDecl(dmod, module, out td);
 			module.TopLevelDecls.Add(td); 
 			break;
 		}
-		case 90: {
+		case 91: {
 			IteratorDecl(dmod, module, out iter);
 			module.TopLevelDecls.Add(iter); 
 			break;
@@ -815,12 +815,12 @@ int StringToInt(string s, int defaultValue, string errString) {
 			module.TopLevelDecls.Add(trait); 
 			break;
 		}
-		case 41: case 42: case 43: case 44: case 45: case 46: case 84: case 85: case 93: case 94: case 95: case 96: {
+		case 41: case 42: case 43: case 44: case 45: case 46: case 84: case 85: case 94: case 95: case 96: case 97: {
 			ClassMemberDecl(dmod, membersDefaultClass, false, !DafnyOptions.O.AllowGlobals, 
 !isTopLevel && DafnyOptions.O.IronDafny && isAbstract);
 			break;
 		}
-		default: SynErr(150); break;
+		default: SynErr(151); break;
 		}
 	}
 
@@ -847,7 +847,7 @@ int StringToInt(string s, int defaultValue, string errString) {
 				dmod.ExternName = new StringLiteralExpr(t, s, isVerbatimString);
 				
 			}
-		} else SynErr(151);
+		} else SynErr(152);
 	}
 
 	void SubModuleDecl(DeclModifierData dmod, ModuleDefinition parent, out ModuleDecl submodule) {
@@ -911,9 +911,9 @@ int StringToInt(string s, int defaultValue, string errString) {
 				Get();
 				QualifiedModuleExport(out idPath, out idExports);
 				submodule = new ModuleFacadeDecl(idPath, id, parent, opened, idExports); 
-			} else SynErr(152);
+			} else SynErr(153);
 			if (la.kind == 30) {
-				while (!(la.kind == 0 || la.kind == 30)) {SynErr(153); Get();}
+				while (!(la.kind == 0 || la.kind == 30)) {SynErr(154); Get();}
 				Get();
 				errors.Deprecated(t, "the semi-colon that used to terminate a sub-module declaration has been deprecated; in the new syntax, just leave off the semi-colon"); 
 			}
@@ -945,7 +945,7 @@ int StringToInt(string s, int defaultValue, string errString) {
 					} else if (la.kind == 61) {
 						Get();
 						provideAll = true; 
-					} else SynErr(154);
+					} else SynErr(155);
 				} else if (la.kind == 78) {
 					Get();
 					if (la.kind == 1) {
@@ -959,7 +959,7 @@ int StringToInt(string s, int defaultValue, string errString) {
 					} else if (la.kind == 61) {
 						Get();
 						revealAll = true; 
-					} else SynErr(155);
+					} else SynErr(156);
 				} else {
 					Get();
 					ModuleExport(out id);
@@ -976,7 +976,7 @@ int StringToInt(string s, int defaultValue, string errString) {
 			}
 			submodule = new ModuleExportDecl(exportId, parent, exports, extends, provideAll, revealAll, isDefault);
 			
-		} else SynErr(156);
+		} else SynErr(157);
 	}
 
 	void ClassDecl(DeclModifierData dmodClass, ModuleDefinition/*!*/ module, out ClassDecl/*!*/ c) {
@@ -992,7 +992,7 @@ int StringToInt(string s, int defaultValue, string errString) {
 		CheckDeclModifiers(dmodClass, "Classes", AllowedDeclModifiers.Extern);
 		DeclModifierData dmod; 
 		
-		while (!(la.kind == 0 || la.kind == 80)) {SynErr(157); Get();}
+		while (!(la.kind == 0 || la.kind == 80)) {SynErr(158); Get();}
 		Expect(80);
 		while (la.kind == 50) {
 			Attribute(ref attrs);
@@ -1039,13 +1039,13 @@ int StringToInt(string s, int defaultValue, string errString) {
 		bool co = false;
 		CheckDeclModifiers(dmod, "Datatypes or codatatypes", AllowedDeclModifiers.None);
 		
-		while (!(la.kind == 0 || la.kind == 82 || la.kind == 83)) {SynErr(158); Get();}
+		while (!(la.kind == 0 || la.kind == 82 || la.kind == 83)) {SynErr(159); Get();}
 		if (la.kind == 82) {
 			Get();
 		} else if (la.kind == 83) {
 			Get();
 			co = true; 
-		} else SynErr(159);
+		} else SynErr(160);
 		while (la.kind == 50) {
 			Attribute(ref attrs);
 		}
@@ -1064,7 +1064,7 @@ int StringToInt(string s, int defaultValue, string errString) {
 			DatatypeMemberDecl(ctors);
 		}
 		if (la.kind == 30) {
-			while (!(la.kind == 0 || la.kind == 30)) {SynErr(160); Get();}
+			while (!(la.kind == 0 || la.kind == 30)) {SynErr(161); Get();}
 			Get();
 			errors.Deprecated(t, "the semi-colon that used to terminate a (co)datatype declaration has been deprecated; in the new syntax, just leave off the semi-colon"); 
 		}
@@ -1083,7 +1083,8 @@ int StringToInt(string s, int defaultValue, string errString) {
 		Attributes attrs = null;
 		td = null;
 		Type baseType = null;
-		Expression wh;
+		Expression constraint;
+		Expression witness = null;
 		CheckDeclModifiers(dmod, "Newtypes", AllowedDeclModifiers.None);
 		
 		Expect(87);
@@ -1100,12 +1101,16 @@ int StringToInt(string s, int defaultValue, string errString) {
 			}
 			if (baseType == null) { baseType = new InferredTypeProxy(); } 
 			Expect(24);
-			Expression(out wh, false, true);
-			td = new NewtypeDecl(id, id.val, module, new BoundVar(bvId, bvId.val, baseType), wh, attrs); 
+			Expression(out constraint, false, true);
+			if (la.kind == 88) {
+				Get();
+				Expression(out witness, false, true);
+			}
+			td = new NewtypeDecl(id, id.val, module, new BoundVar(bvId, bvId.val, baseType), constraint, witness, attrs); 
 		} else if (StartOf(6)) {
 			Type(out baseType);
 			td = new NewtypeDecl(id, id.val, module, baseType, attrs); 
-		} else SynErr(161);
+		} else SynErr(162);
 	}
 
 	void OtherTypeDecl(DeclModifierData dmod, ModuleDefinition module, out TopLevelDecl td) {
@@ -1116,9 +1121,10 @@ int StringToInt(string s, int defaultValue, string errString) {
 		td = null;
 		Type ty = null;
 		Expression constraint;
+		Expression witness = null;
 		var kind = "Opaque type";
 		
-		Expect(88);
+		Expect(89);
 		while (la.kind == 50) {
 			Attribute(ref attrs);
 		}
@@ -1143,7 +1149,11 @@ int StringToInt(string s, int defaultValue, string errString) {
 				if (ty == null) { ty = new InferredTypeProxy(); } 
 				Expect(24);
 				Expression(out constraint, false, true);
-				td = new SubsetTypeDecl(id, id.val, eqSupport, typeArgs, module, new BoundVar(bvId, bvId.val, ty), constraint, attrs);
+				if (la.kind == 88) {
+					Get();
+					Expression(out witness, false, true);
+				}
+				td = new SubsetTypeDecl(id, id.val, eqSupport, typeArgs, module, new BoundVar(bvId, bvId.val, ty), constraint, witness, attrs);
 				kind = "Subset type";
 				
 			} else if (StartOf(6)) {
@@ -1151,7 +1161,7 @@ int StringToInt(string s, int defaultValue, string errString) {
 				td = new TypeSynonymDecl(id, id.val, eqSupport, typeArgs, module, ty, attrs);
 				kind = "Type synonym";
 				
-			} else SynErr(162);
+			} else SynErr(163);
 		}
 		if (td == null) {
 		 td = new OpaqueTypeDecl(id, id.val, module, eqSupport, typeArgs, attrs);
@@ -1159,7 +1169,7 @@ int StringToInt(string s, int defaultValue, string errString) {
 		
 		CheckDeclModifiers(dmod, kind, AllowedDeclModifiers.None); 
 		if (la.kind == 30) {
-			while (!(la.kind == 0 || la.kind == 30)) {SynErr(163); Get();}
+			while (!(la.kind == 0 || la.kind == 30)) {SynErr(164); Get();}
 			Get();
 			errors.Deprecated(t, "the semi-colon that used to terminate an opaque-type declaration has been deprecated; in the new syntax, just leave off the semi-colon"); 
 		}
@@ -1189,8 +1199,8 @@ int StringToInt(string s, int defaultValue, string errString) {
 		IToken bodyEnd = Token.NoToken;
 		CheckDeclModifiers(dmod, "Iterators", AllowedDeclModifiers.None);
 		
-		while (!(la.kind == 0 || la.kind == 90)) {SynErr(164); Get();}
-		Expect(90);
+		while (!(la.kind == 0 || la.kind == 91)) {SynErr(165); Get();}
+		Expect(91);
 		while (la.kind == 50) {
 			Attribute(ref attrs);
 		}
@@ -1200,8 +1210,8 @@ int StringToInt(string s, int defaultValue, string errString) {
 				GenericParameters(typeArgs);
 			}
 			Formals(true, true, false, ins);
-			if (la.kind == 91 || la.kind == 92) {
-				if (la.kind == 91) {
+			if (la.kind == 92 || la.kind == 93) {
+				if (la.kind == 92) {
 					Get();
 				} else {
 					Get();
@@ -1212,7 +1222,7 @@ int StringToInt(string s, int defaultValue, string errString) {
 		} else if (la.kind == 63) {
 			Get();
 			signatureEllipsis = t; 
-		} else SynErr(165);
+		} else SynErr(166);
 		while (StartOf(7)) {
 			IteratorSpec(reads, mod, decreases, req, ens, yieldReq, yieldEns, ref readsAttrs, ref modAttrs, ref decrAttrs);
 		}
@@ -1241,7 +1251,7 @@ int StringToInt(string s, int defaultValue, string errString) {
 		IToken bodyStart;
 		DeclModifierData dmod; 
 		
-		while (!(la.kind == 0 || la.kind == 81)) {SynErr(166); Get();}
+		while (!(la.kind == 0 || la.kind == 81)) {SynErr(167); Get();}
 		Expect(81);
 		while (la.kind == 50) {
 			Attribute(ref attrs);
@@ -1296,7 +1306,7 @@ int StringToInt(string s, int defaultValue, string errString) {
 			
 			MethodDecl(dmod, allowConstructors, isWithinAbstractModule, out m);
 			mm.Add(m); 
-		} else SynErr(167);
+		} else SynErr(168);
 	}
 
 	void Attribute(ref Attributes attrs) {
@@ -1358,8 +1368,8 @@ int StringToInt(string s, int defaultValue, string errString) {
 					exports.Add(id); 
 				}
 				Expect(51);
-			} else SynErr(168);
-		} else SynErr(169);
+			} else SynErr(169);
+		} else SynErr(170);
 	}
 
 	void QualifiedModuleExport(out List<IToken> ids, out List<IToken> exports) {
@@ -1441,7 +1451,7 @@ int StringToInt(string s, int defaultValue, string errString) {
 		} else if (la.kind == 48) {
 			Get();
 			x = t; 
-		} else SynErr(170);
+		} else SynErr(171);
 	}
 
 	void GenericParameters(List<TypeParameter/*!*/>/*!*/ typeArgs) {
@@ -1485,7 +1495,7 @@ int StringToInt(string s, int defaultValue, string errString) {
 		IToken/*!*/ id;  Type/*!*/ ty;
 		CheckDeclModifiers(dmod, "Fields", AllowedDeclModifiers.Ghost);
 		
-		while (!(la.kind == 0 || la.kind == 84)) {SynErr(171); Get();}
+		while (!(la.kind == 0 || la.kind == 84)) {SynErr(172); Get();}
 		Expect(84);
 		while (la.kind == 50) {
 			Attribute(ref attrs);
@@ -1506,7 +1516,7 @@ int StringToInt(string s, int defaultValue, string errString) {
 		IToken/*!*/ id;  Type/*!*/ ty; Expression/*!*/ e;
 		CheckDeclModifiers(dmod, "Fields", AllowedDeclModifiers.Ghost);
 		
-		while (!(la.kind == 0 || la.kind == 85)) {SynErr(172); Get();}
+		while (!(la.kind == 0 || la.kind == 85)) {SynErr(173); Get();}
 		Expect(85);
 		while (la.kind == 50) {
 			Attribute(ref attrs);
@@ -1545,7 +1555,7 @@ int StringToInt(string s, int defaultValue, string errString) {
 		}
 		if (la.kind == 41) {
 			Get();
-			if (la.kind == 93) {
+			if (la.kind == 94) {
 				Get();
 				if (isTwoState) { SemErr(t, "twostate functions are supported only as a ghosts, not as function methods"); }
 				else { isFunctionMethod = true; }
@@ -1582,15 +1592,15 @@ int StringToInt(string s, int defaultValue, string errString) {
 					Expect(55);
 				} else if (StartOf(6)) {
 					Type(out returnType);
-				} else SynErr(173);
+				} else SynErr(174);
 			} else if (la.kind == 63) {
 				Get();
 				signatureEllipsis = t; 
-			} else SynErr(174);
+			} else SynErr(175);
 		} else if (la.kind == 42) {
 			Get();
 			isPredicate = true; 
-			if (la.kind == 93) {
+			if (la.kind == 94) {
 				Get();
 				if (isTwoState) { SemErr(t, "twostate predicates are supported only as a ghosts, not as predicate methods"); }
 				else { isFunctionMethod = true; }
@@ -1626,7 +1636,7 @@ int StringToInt(string s, int defaultValue, string errString) {
 			} else if (la.kind == 63) {
 				Get();
 				signatureEllipsis = t; 
-			} else SynErr(175);
+			} else SynErr(176);
 		} else if (la.kind == 43) {
 			Contract.Assert(!isTwoState);  // the IsFunctionDecl check checks that "twostate" is not followed by "inductive"
 			
@@ -1652,7 +1662,7 @@ int StringToInt(string s, int defaultValue, string errString) {
 			} else if (la.kind == 63) {
 				Get();
 				signatureEllipsis = t; 
-			} else SynErr(176);
+			} else SynErr(177);
 		} else if (la.kind == 46) {
 			Contract.Assert(!isTwoState);  // the IsFunctionDecl check checks that "twostate" is not followed by "copredicate"
 			
@@ -1677,8 +1687,8 @@ int StringToInt(string s, int defaultValue, string errString) {
 			} else if (la.kind == 63) {
 				Get();
 				signatureEllipsis = t; 
-			} else SynErr(177);
-		} else SynErr(178);
+			} else SynErr(178);
+		} else SynErr(179);
 		decreases = isIndPredicate || isCoPredicate ? null : new List<Expression/*!*/>(); 
 		while (StartOf(11)) {
 			FunctionSpec(reqs, reads, ens, decreases);
@@ -1748,9 +1758,9 @@ int StringToInt(string s, int defaultValue, string errString) {
 		AllowedDeclModifiers allowed = AllowedDeclModifiers.None;
 		string caption = "";
 		
-		while (!(StartOf(12))) {SynErr(179); Get();}
+		while (!(StartOf(12))) {SynErr(180); Get();}
 		switch (la.kind) {
-		case 93: {
+		case 94: {
 			Get();
 			isPlainOlMethod = true; caption = "Methods";
 			allowed = AllowedDeclModifiers.Ghost | AllowedDeclModifiers.Static 
@@ -1764,14 +1774,14 @@ int StringToInt(string s, int defaultValue, string errString) {
 			 | AllowedDeclModifiers.Protected; 
 			break;
 		}
-		case 94: {
+		case 95: {
 			Get();
 			isCoLemma = true; caption = "Colemmas";
 			allowed = AllowedDeclModifiers.AlreadyGhost | AllowedDeclModifiers.Static 
 			 | AllowedDeclModifiers.Protected; 
 			break;
 		}
-		case 95: {
+		case 96: {
 			Get();
 			isCoLemma = true; caption = "Comethods";
 			allowed = AllowedDeclModifiers.AlreadyGhost | AllowedDeclModifiers.Static 
@@ -1795,7 +1805,7 @@ int StringToInt(string s, int defaultValue, string errString) {
 			 | AllowedDeclModifiers.Protected; 
 			break;
 		}
-		case 96: {
+		case 97: {
 			Get();
 			if (allowConstructor) {
 			 isConstructor = true;
@@ -1807,7 +1817,7 @@ int StringToInt(string s, int defaultValue, string errString) {
 			
 			break;
 		}
-		default: SynErr(180); break;
+		default: SynErr(181); break;
 		}
 		keywordToken = t; 
 		CheckDeclModifiers(dmod, caption, allowed); 
@@ -1832,7 +1842,7 @@ int StringToInt(string s, int defaultValue, string errString) {
 			}
 			var isCompilable = (isPlainOlMethod && !dmod.IsGhost) || isConstructor; 
 			Formals(true, isCompilable, isTwoStateLemma, ins);
-			if (la.kind == 92) {
+			if (la.kind == 93) {
 				Get();
 				if (isConstructor) { SemErr(t, "constructors cannot have out-parameters"); } 
 				Formals(false, isCompilable, false, outs);
@@ -1840,7 +1850,7 @@ int StringToInt(string s, int defaultValue, string errString) {
 		} else if (la.kind == 63) {
 			Get();
 			signatureEllipsis = t; 
-		} else SynErr(181);
+		} else SynErr(182);
 		while (StartOf(13)) {
 			MethodSpec(req, mod, ens, dec, ref decAttrs, ref modAttrs, caption);
 		}
@@ -1917,14 +1927,14 @@ int StringToInt(string s, int defaultValue, string errString) {
 		} else if (la.kind == 2) {
 			Get();
 			id = t; 
-		} else SynErr(182);
+		} else SynErr(183);
 		Expect(22);
 		Type(out ty);
 	}
 
 	void OldSemi() {
 		if (la.kind == 30) {
-			while (!(la.kind == 0 || la.kind == 30)) {SynErr(183); Get();}
+			while (!(la.kind == 0 || la.kind == 30)) {SynErr(184); Get();}
 			Get();
 			errors.DeprecatedStyle(t, "deprecated style: a semi-colon is not needed here"); 
 		}
@@ -1948,7 +1958,7 @@ int StringToInt(string s, int defaultValue, string errString) {
 		Contract.Ensures(Contract.ValueAtReturn(out id)!=null);
 		Contract.Ensures(Contract.ValueAtReturn(out ty)!=null);
 		isGhost = false; isOld = allowNewKeyword; 
-		while (la.kind == 67 || la.kind == 89) {
+		while (la.kind == 67 || la.kind == 90) {
 			if (la.kind == 67) {
 				Get();
 				if (allowGhostKeyword) { isGhost = true; } else { SemErr(t, "formal cannot be declared 'ghost' in this context"); } 
@@ -2027,7 +2037,7 @@ int StringToInt(string s, int defaultValue, string errString) {
 			id = t; name = id.val;
 			Expect(22);
 			Type(out ty);
-		} else SynErr(184);
+		} else SynErr(185);
 		if (name != null) {
 		 identName = name;
 		} else {
@@ -2205,7 +2215,7 @@ int StringToInt(string s, int defaultValue, string errString) {
 			ty = new UserDefinedType(e.tok, e); 
 			break;
 		}
-		default: SynErr(185); break;
+		default: SynErr(186); break;
 		}
 		if (IsArrow()) {
 			Expect(32);
@@ -2230,7 +2240,7 @@ int StringToInt(string s, int defaultValue, string errString) {
 		bool isOld;
 		
 		Expect(54);
-		if (la.kind == 1 || la.kind == 67 || la.kind == 89) {
+		if (la.kind == 1 || la.kind == 67 || la.kind == 90) {
 			GIdentType(allowGhostKeyword, allowNewKeyword, out id, out ty, out isGhost, out isOld);
 			formals.Add(new Formal(id, id.val, ty, incoming, isGhost, isOld)); 
 			while (la.kind == 23) {
@@ -2248,7 +2258,7 @@ List<MaybeFreeExpression/*!*/>/*!*/ yieldReq, List<MaybeFreeExpression/*!*/>/*!*
 ref Attributes readsAttrs, ref Attributes modAttrs, ref Attributes decrAttrs) {
 		Expression/*!*/ e; FrameExpression/*!*/ fe; bool isFree = false; bool isYield = false; Attributes ensAttrs = null;
 		
-		while (!(StartOf(15))) {SynErr(186); Get();}
+		while (!(StartOf(15))) {SynErr(187); Get();}
 		if (la.kind == 48) {
 			Get();
 			while (IsAttribute()) {
@@ -2276,13 +2286,13 @@ ref Attributes readsAttrs, ref Attributes modAttrs, ref Attributes decrAttrs) {
 			}
 			OldSemi();
 		} else if (StartOf(16)) {
-			if (la.kind == 97) {
+			if (la.kind == 98) {
 				Get();
 				isFree = true;
 				errors.Deprecated(t, "the 'free' keyword is soon to be deprecated");
 				
 			}
-			if (la.kind == 99) {
+			if (la.kind == 100) {
 				Get();
 				isYield = true; 
 			}
@@ -2296,7 +2306,7 @@ ref Attributes readsAttrs, ref Attributes modAttrs, ref Attributes decrAttrs) {
 				 req.Add(new MaybeFreeExpression(e, isFree));
 				}
 				
-			} else if (la.kind == 98) {
+			} else if (la.kind == 99) {
 				Get();
 				while (IsAttribute()) {
 					Attribute(ref ensAttrs);
@@ -2309,7 +2319,7 @@ ref Attributes readsAttrs, ref Attributes modAttrs, ref Attributes decrAttrs) {
 				 ens.Add(new MaybeFreeExpression(e, isFree, ensAttrs));
 				}
 				
-			} else SynErr(187);
+			} else SynErr(188);
 		} else if (la.kind == 39) {
 			Get();
 			while (IsAttribute()) {
@@ -2317,7 +2327,7 @@ ref Attributes readsAttrs, ref Attributes modAttrs, ref Attributes decrAttrs) {
 			}
 			DecreasesList(decreases, false, false);
 			OldSemi();
-		} else SynErr(188);
+		} else SynErr(189);
 	}
 
 	void BlockStmt(out BlockStmt/*!*/ block, out IToken bodyStart, out IToken bodyEnd) {
@@ -2342,7 +2352,7 @@ List<Expression> decreases, ref Attributes decAttrs, ref Attributes modAttrs, st
 		Contract.Requires(cce.NonNullElements(decreases));
 		Expression e;  FrameExpression fe;  bool isFree = false; Attributes ensAttrs = null;
 		
-		while (!(StartOf(18))) {SynErr(189); Get();}
+		while (!(StartOf(18))) {SynErr(190); Get();}
 		if (la.kind == 47) {
 			Get();
 			while (IsAttribute()) {
@@ -2356,8 +2366,8 @@ List<Expression> decreases, ref Attributes decAttrs, ref Attributes modAttrs, st
 				mod.Add(fe); 
 			}
 			OldSemi();
-		} else if (la.kind == 49 || la.kind == 97 || la.kind == 98) {
-			if (la.kind == 97) {
+		} else if (la.kind == 49 || la.kind == 98 || la.kind == 99) {
+			if (la.kind == 98) {
 				Get();
 				isFree = true;
 				errors.Deprecated(t, "the 'free' keyword is soon to be deprecated");
@@ -2368,7 +2378,7 @@ List<Expression> decreases, ref Attributes decAttrs, ref Attributes modAttrs, st
 				Expression(out e, false, false);
 				OldSemi();
 				req.Add(new MaybeFreeExpression(e, isFree)); 
-			} else if (la.kind == 98) {
+			} else if (la.kind == 99) {
 				Get();
 				while (IsAttribute()) {
 					Attribute(ref ensAttrs);
@@ -2376,7 +2386,7 @@ List<Expression> decreases, ref Attributes decAttrs, ref Attributes modAttrs, st
 				Expression(out e, false, false);
 				OldSemi();
 				ens.Add(new MaybeFreeExpression(e, isFree, ensAttrs)); 
-			} else SynErr(190);
+			} else SynErr(191);
 		} else if (la.kind == 39) {
 			Get();
 			while (IsAttribute()) {
@@ -2384,7 +2394,7 @@ List<Expression> decreases, ref Attributes decAttrs, ref Attributes modAttrs, st
 			}
 			DecreasesList(decreases, true, false);
 			OldSemi();
-		} else SynErr(191);
+		} else SynErr(192);
 	}
 
 	void FrameExpression(out FrameExpression fe, bool allowSemi, bool allowLambda) {
@@ -2408,7 +2418,7 @@ List<Expression> decreases, ref Attributes decAttrs, ref Attributes modAttrs, st
 			Ident(out id);
 			fieldName = id.val; 
 			fe = new FrameExpression(id, new ImplicitThisExpr(id), fieldName); 
-		} else SynErr(192);
+		} else SynErr(193);
 	}
 
 	void DecreasesList(List<Expression> decreases, bool allowWildcard, bool allowLambda) {
@@ -2466,7 +2476,7 @@ List<Expression> decreases, ref Attributes decAttrs, ref Attributes modAttrs, st
 		Contract.Requires(cce.NonNullElements(reads));
 		Contract.Requires(decreases == null || cce.NonNullElements(decreases));
 		Expression/*!*/ e;  FrameExpression/*!*/ fe; 
-		while (!(StartOf(19))) {SynErr(193); Get();}
+		while (!(StartOf(19))) {SynErr(194); Get();}
 		if (la.kind == 49) {
 			Get();
 			Expression(out e, false, false);
@@ -2482,7 +2492,7 @@ List<Expression> decreases, ref Attributes decAttrs, ref Attributes modAttrs, st
 				reads.Add(fe); 
 			}
 			OldSemi();
-		} else if (la.kind == 98) {
+		} else if (la.kind == 99) {
 			Get();
 			Expression(out e, false, false);
 			OldSemi();
@@ -2496,7 +2506,7 @@ List<Expression> decreases, ref Attributes decAttrs, ref Attributes modAttrs, st
 			
 			DecreasesList(decreases, false, false);
 			OldSemi();
-		} else SynErr(194);
+		} else SynErr(195);
 	}
 
 	void FunctionBody(out Expression/*!*/ e, out IToken bodyStart, out IToken bodyEnd) {
@@ -2515,7 +2525,7 @@ List<Expression> decreases, ref Attributes decAttrs, ref Attributes modAttrs, st
 			fe = new FrameExpression(t, new WildcardExpr(t), null); 
 		} else if (StartOf(20)) {
 			FrameExpression(out fe, allowSemi, false);
-		} else SynErr(195);
+		} else SynErr(196);
 	}
 
 	void PossiblyWildExpression(out Expression e, bool allowLambda) {
@@ -2526,7 +2536,7 @@ List<Expression> decreases, ref Attributes decAttrs, ref Attributes modAttrs, st
 			e = new WildcardExpr(t); 
 		} else if (StartOf(9)) {
 			Expression(out e, false, allowLambda);
-		} else SynErr(196);
+		} else SynErr(197);
 	}
 
 	void Stmt(List<Statement/*!*/>/*!*/ ss) {
@@ -2543,14 +2553,14 @@ List<Expression> decreases, ref Attributes decAttrs, ref Attributes modAttrs, st
 		IToken bodyStart, bodyEnd;
 		int breakCount;
 		
-		while (!(StartOf(21))) {SynErr(197); Get();}
+		while (!(StartOf(21))) {SynErr(198); Get();}
 		switch (la.kind) {
 		case 50: {
 			BlockStmt(out bs, out bodyStart, out bodyEnd);
 			s = bs; 
 			break;
 		}
-		case 107: {
+		case 108: {
 			AssertStmt(out s);
 			break;
 		}
@@ -2558,7 +2568,7 @@ List<Expression> decreases, ref Attributes decAttrs, ref Attributes modAttrs, st
 			AssumeStmt(out s);
 			break;
 		}
-		case 109: {
+		case 110: {
 			PrintStmt(out s);
 			break;
 		}
@@ -2566,7 +2576,7 @@ List<Expression> decreases, ref Attributes decAttrs, ref Attributes modAttrs, st
 			RevealStmt(out s);
 			break;
 		}
-		case 1: case 2: case 3: case 4: case 9: case 11: case 20: case 21: case 24: case 54: case 140: case 141: case 142: case 143: case 144: case 145: case 146: case 147: {
+		case 1: case 2: case 3: case 4: case 9: case 11: case 20: case 21: case 24: case 54: case 141: case 142: case 143: case 144: case 145: case 146: case 147: case 148: {
 			UpdateStmt(out s);
 			break;
 		}
@@ -2574,19 +2584,19 @@ List<Expression> decreases, ref Attributes decAttrs, ref Attributes modAttrs, st
 			VarDeclStatement(out s);
 			break;
 		}
-		case 104: {
+		case 105: {
 			IfStmt(out s);
 			break;
 		}
-		case 105: {
+		case 106: {
 			WhileStmt(out s);
 			break;
 		}
-		case 106: {
+		case 107: {
 			MatchStmt(out s);
 			break;
 		}
-		case 110: case 111: {
+		case 111: case 112: {
 			ForallStmt(out s);
 			break;
 		}
@@ -2594,11 +2604,11 @@ List<Expression> decreases, ref Attributes decAttrs, ref Attributes modAttrs, st
 			CalcStmt(out s);
 			break;
 		}
-		case 112: {
+		case 113: {
 			ModifyStmt(out s);
 			break;
 		}
-		case 100: {
+		case 101: {
 			Get();
 			x = t; 
 			NoUSIdent(out id);
@@ -2607,24 +2617,24 @@ List<Expression> decreases, ref Attributes decAttrs, ref Attributes modAttrs, st
 			s.Labels = new LList<Label>(new Label(x, id.val), s.Labels); 
 			break;
 		}
-		case 101: {
+		case 102: {
 			Get();
 			x = t; breakCount = 1; label = null; 
 			if (la.kind == 1) {
 				NoUSIdent(out id);
 				label = id.val; 
-			} else if (la.kind == 30 || la.kind == 101) {
-				while (la.kind == 101) {
+			} else if (la.kind == 30 || la.kind == 102) {
+				while (la.kind == 102) {
 					Get();
 					breakCount++; 
 				}
-			} else SynErr(198);
-			while (!(la.kind == 0 || la.kind == 30)) {SynErr(199); Get();}
+			} else SynErr(199);
+			while (!(la.kind == 0 || la.kind == 30)) {SynErr(200); Get();}
 			Expect(30);
 			s = label != null ? new BreakStmt(x, t, label) : new BreakStmt(x, t, breakCount); 
 			break;
 		}
-		case 99: case 103: {
+		case 100: case 104: {
 			ReturnStmt(out s);
 			break;
 		}
@@ -2632,7 +2642,7 @@ List<Expression> decreases, ref Attributes decAttrs, ref Attributes modAttrs, st
 			SkeletonStmt(out s);
 			break;
 		}
-		default: SynErr(200); break;
+		default: SynErr(201); break;
 		}
 	}
 
@@ -2643,24 +2653,24 @@ List<Expression> decreases, ref Attributes decAttrs, ref Attributes modAttrs, st
 		BlockStmt proof = null;
 		IToken proofStart, proofEnd;
 		
-		Expect(107);
+		Expect(108);
 		x = t; 
 		while (IsAttribute()) {
 			Attribute(ref attrs);
 		}
 		if (StartOf(9)) {
 			Expression(out e, false, true);
-			if (la.kind == 108) {
+			if (la.kind == 109) {
 				Get();
 				BlockStmt(out proof, out proofStart, out proofEnd);
 			} else if (la.kind == 30) {
 				Get();
-			} else SynErr(201);
+			} else SynErr(202);
 		} else if (la.kind == 63) {
 			Get();
 			dotdotdot = t; 
 			Expect(30);
-		} else SynErr(202);
+		} else SynErr(203);
 		if (dotdotdot != null) {
 		 s = new SkeletonStatement(new AssertStmt(x, t, new LiteralExpr(x, true), null, attrs), dotdotdot, null);
 		} else {
@@ -2684,7 +2694,7 @@ List<Expression> decreases, ref Attributes decAttrs, ref Attributes modAttrs, st
 		} else if (la.kind == 63) {
 			Get();
 			dotdotdot = t; 
-		} else SynErr(203);
+		} else SynErr(204);
 		Expect(30);
 		if (dotdotdot != null) {
 		 s = new SkeletonStatement(new AssumeStmt(x, t, new LiteralExpr(x, true), attrs), dotdotdot, null);
@@ -2699,7 +2709,7 @@ List<Expression> decreases, ref Attributes decAttrs, ref Attributes modAttrs, st
 		IToken x;  Expression e;
 		var args = new List<Expression>();
 		
-		Expect(109);
+		Expect(110);
 		x = t; 
 		Expression(out e, false, true);
 		args.Add(e); 
@@ -2765,13 +2775,13 @@ List<Expression> decreases, ref Attributes decAttrs, ref Attributes modAttrs, st
 					suchThatAssume = t; 
 				}
 				Expression(out suchThat, false, true);
-			} else SynErr(204);
+			} else SynErr(205);
 			Expect(30);
 			endTok = t; 
 		} else if (la.kind == 22) {
 			Get();
 			SemErr(t, "invalid statement (did you forget the 'label' keyword?)"); 
-		} else SynErr(205);
+		} else SynErr(206);
 		if (suchThat != null) {
 		 s = new AssignSuchThatStmt(x, endTok, lhss, suchThat, suchThatAssume, null);
 		} else {
@@ -2840,7 +2850,7 @@ List<Expression> decreases, ref Attributes decAttrs, ref Attributes modAttrs, st
 					Expression(out suchThat, false, true);
 				}
 			}
-			while (!(la.kind == 0 || la.kind == 30)) {SynErr(206); Get();}
+			while (!(la.kind == 0 || la.kind == 30)) {SynErr(207); Get();}
 			Expect(30);
 			endTok = t; 
 			ConcreteUpdateStatement update;
@@ -2894,12 +2904,12 @@ List<Expression> decreases, ref Attributes decAttrs, ref Attributes modAttrs, st
 				}
 				Expect(26);
 				SemErr(pat.tok, "LHS of assign-such-that expression must be variables, not general patterns"); 
-			} else SynErr(207);
+			} else SynErr(208);
 			Expression(out e, false, true);
 			letRHSs.Add(e); 
 			Expect(30);
 			s = new LetStmt(e.tok, e.tok, letLHSs, letRHSs); 
-		} else SynErr(208);
+		} else SynErr(209);
 	}
 
 	void IfStmt(out Statement/*!*/ ifStmt) {
@@ -2914,7 +2924,7 @@ List<Expression> decreases, ref Attributes decAttrs, ref Attributes modAttrs, st
 		ifStmt = dummyStmt;  // to please the compiler
 		bool usesOptionalBraces;
 		
-		Expect(104);
+		Expect(105);
 		x = t; 
 		if (IsAlternative()) {
 			AlternativeBlock(true, out alternatives, out usesOptionalBraces, out endTok);
@@ -2933,13 +2943,13 @@ List<Expression> decreases, ref Attributes decAttrs, ref Attributes modAttrs, st
 			endTok = thn.EndTok; 
 			if (la.kind == 37) {
 				Get();
-				if (la.kind == 104) {
+				if (la.kind == 105) {
 					IfStmt(out s);
 					els = s; endTok = s.EndTok; 
 				} else if (la.kind == 50) {
 					BlockStmt(out bs, out bodyStart, out bodyEnd);
 					els = bs; endTok = bs.EndTok; 
-				} else SynErr(209);
+				} else SynErr(210);
 			}
 			if (guardEllipsis != null) {
 			 ifStmt = new SkeletonStatement(new IfStmt(x, endTok, isExistentialGuard, guard, thn, els), guardEllipsis, null);
@@ -2947,7 +2957,7 @@ List<Expression> decreases, ref Attributes decAttrs, ref Attributes modAttrs, st
 			 ifStmt = new IfStmt(x, endTok, isExistentialGuard, guard, thn, els);
 			}
 			
-		} else SynErr(210);
+		} else SynErr(211);
 	}
 
 	void WhileStmt(out Statement stmt) {
@@ -2967,7 +2977,7 @@ List<Expression> decreases, ref Attributes decAttrs, ref Attributes modAttrs, st
 		bool isDirtyLoop = true;
 		bool usesOptionalBraces;
 		
-		Expect(105);
+		Expect(106);
 		x = t; 
 		if (IsLoopSpec() || IsAlternative()) {
 			while (StartOf(24)) {
@@ -2993,7 +3003,7 @@ List<Expression> decreases, ref Attributes decAttrs, ref Attributes modAttrs, st
 				Expect(63);
 				bodyEllipsis = t; endTok = t; isDirtyLoop = false; 
 			} else if (StartOf(25)) {
-			} else SynErr(211);
+			} else SynErr(212);
 			if (guardEllipsis != null || bodyEllipsis != null) {
 			 if (mod != null) {
 			   SemErr(mod[0].E.tok, "'modifies' clauses are not allowed on refining loops");
@@ -3011,7 +3021,7 @@ List<Expression> decreases, ref Attributes decAttrs, ref Attributes modAttrs, st
 			 stmt = new WhileStmt(x, endTok, guard, invariants, new Specification<Expression>(decreases, decAttrs), new Specification<FrameExpression>(mod, modAttrs), body);
 			}
 			
-		} else SynErr(212);
+		} else SynErr(213);
 	}
 
 	void MatchStmt(out Statement/*!*/ s) {
@@ -3020,7 +3030,7 @@ List<Expression> decreases, ref Attributes decAttrs, ref Attributes modAttrs, st
 		List<MatchCaseStmt/*!*/> cases = new List<MatchCaseStmt/*!*/>();
 		bool usesOptionalBraces = false;
 		
-		Expect(106);
+		Expect(107);
 		x = t; 
 		Expression(out e, true, true);
 		if (la.kind == _lbrace) {
@@ -3036,7 +3046,7 @@ List<Expression> decreases, ref Attributes decAttrs, ref Attributes modAttrs, st
 				CaseStatement(out c);
 				cases.Add(c); 
 			}
-		} else SynErr(213);
+		} else SynErr(214);
 		s = new MatchStmt(x, t, e, cases, usesOptionalBraces); 
 	}
 
@@ -3053,15 +3063,15 @@ List<Expression> decreases, ref Attributes decAttrs, ref Attributes modAttrs, st
 		IToken bodyStart, bodyEnd;
 		IToken tok = Token.NoToken;
 		
-		if (la.kind == 110) {
+		if (la.kind == 111) {
 			Get();
 			x = t; tok = x; 
-		} else if (la.kind == 111) {
+		} else if (la.kind == 112) {
 			Get();
 			x = t;
 			errors.Deprecated(t, "the 'parallel' keyword has been deprecated; the comprehension statement now uses the keyword 'forall' (and the parentheses around the bound variables are now optional)");
 			
-		} else SynErr(214);
+		} else SynErr(215);
 		if (la.kind == _openparen) {
 			Expect(54);
 			if (la.kind == 1) {
@@ -3072,19 +3082,19 @@ List<Expression> decreases, ref Attributes decAttrs, ref Attributes modAttrs, st
 			if (la.kind == _ident) {
 				QuantifierDomain(out bvars, out attrs, out range);
 			}
-		} else SynErr(215);
+		} else SynErr(216);
 		if (bvars == null) { bvars = new List<BoundVar>(); }
 		if (range == null) { range = new LiteralExpr(x, true); }
 		
-		while (la.kind == 97 || la.kind == 98) {
+		while (la.kind == 98 || la.kind == 99) {
 			isFree = false; 
-			if (la.kind == 97) {
+			if (la.kind == 98) {
 				Get();
 				isFree = true;
 				errors.Deprecated(t, "the 'free' keyword is soon to be deprecated");
 				
 			}
-			Expect(98);
+			Expect(99);
 			Expression(out e, false, true);
 			ens.Add(new MaybeFreeExpression(e, isFree)); 
 			OldSemi();
@@ -3162,7 +3172,7 @@ List<Expression> decreases, ref Attributes decAttrs, ref Attributes modAttrs, st
 				} else if (la.kind == 34) {
 					CalcStmt(out subCalc);
 					hintEnd = subCalc.EndTok; subhints.Add(subCalc); 
-				} else SynErr(216);
+				} else SynErr(217);
 			}
 			var h = new BlockStmt(hintStart, hintEnd, subhints); // if the hint is empty, hintStart is the first token of the next line, but it doesn't matter because the block statement is just used as a container
 			hints.Add(h);
@@ -3188,7 +3198,7 @@ List<Expression> decreases, ref Attributes decAttrs, ref Attributes modAttrs, st
 		BlockStmt body = null;  IToken bodyStart;
 		IToken ellipsisToken = null;
 		
-		Expect(112);
+		Expect(113);
 		tok = t; 
 		while (IsAttribute()) {
 			Attribute(ref attrs);
@@ -3204,14 +3214,14 @@ List<Expression> decreases, ref Attributes decAttrs, ref Attributes modAttrs, st
 		} else if (la.kind == 63) {
 			Get();
 			ellipsisToken = t; 
-		} else SynErr(217);
+		} else SynErr(218);
 		if (la.kind == 50) {
 			BlockStmt(out body, out bodyStart, out endTok);
 		} else if (la.kind == 30) {
-			while (!(la.kind == 0 || la.kind == 30)) {SynErr(218); Get();}
+			while (!(la.kind == 0 || la.kind == 30)) {SynErr(219); Get();}
 			Get();
 			endTok = t; 
-		} else SynErr(219);
+		} else SynErr(220);
 		s = new ModifyStmt(tok, endTok, mod, attrs, body);
 		if (ellipsisToken != null) {
 		 s = new SkeletonStatement(s, ellipsisToken, null);
@@ -3225,13 +3235,13 @@ List<Expression> decreases, ref Attributes decAttrs, ref Attributes modAttrs, st
 		AssignmentRhs r;
 		bool isYield = false;
 		
-		if (la.kind == 103) {
+		if (la.kind == 104) {
 			Get();
 			returnTok = t; 
-		} else if (la.kind == 99) {
+		} else if (la.kind == 100) {
 			Get();
 			returnTok = t; isYield = true; 
-		} else SynErr(220);
+		} else SynErr(221);
 		if (StartOf(28)) {
 			Rhs(out r);
 			rhss = new List<AssignmentRhs>(); rhss.Add(r); 
@@ -3257,7 +3267,7 @@ List<Expression> decreases, ref Attributes decAttrs, ref Attributes modAttrs, st
 		Expression e; 
 		Expect(63);
 		dotdotdot = t; 
-		if (la.kind == 102) {
+		if (la.kind == 103) {
 			Get();
 			names = new List<IToken>(); exprs = new List<Expression>(); whereTok = t;
 			Ident(out tok);
@@ -3294,7 +3304,7 @@ List<Expression> decreases, ref Attributes decAttrs, ref Attributes modAttrs, st
 		r = dummyRhs;  // to please compiler
 		Attributes attrs = null;
 		
-		if (la.kind == 89) {
+		if (la.kind == 90) {
 			Get();
 			newToken = t; 
 			TypeAndToken(out x, out ty, false);
@@ -3329,7 +3339,7 @@ List<Expression> decreases, ref Attributes decAttrs, ref Attributes modAttrs, st
 		} else if (StartOf(9)) {
 			Expression(out e, false, true);
 			r = new ExprRhs(e); 
-		} else SynErr(221);
+		} else SynErr(222);
 		while (la.kind == 50) {
 			Attribute(ref attrs);
 		}
@@ -3350,7 +3360,7 @@ List<Expression> decreases, ref Attributes decAttrs, ref Attributes modAttrs, st
 			while (la.kind == 28 || la.kind == 52 || la.kind == 54) {
 				Suffix(ref e);
 			}
-		} else SynErr(222);
+		} else SynErr(223);
 	}
 
 	void Expressions(List<Expression> args) {
@@ -3407,7 +3417,7 @@ List<Expression> decreases, ref Attributes decAttrs, ref Attributes modAttrs, st
 			IdentTypeOptional(out bv);
 			pat = new CasePattern(bv.tok, bv);
 			
-		} else SynErr(223);
+		} else SynErr(224);
 		if (pat == null) {
 		 pat = new CasePattern(t, "_ParseError", new List<CasePattern>());
 		}
@@ -3435,7 +3445,7 @@ List<Expression> decreases, ref Attributes decAttrs, ref Attributes modAttrs, st
 				AlternativeBlockCase(allowExistentialGuards, out alt);
 				alternatives.Add(alt); 
 			}
-		} else SynErr(224);
+		} else SynErr(225);
 		endTok = t; 
 	}
 
@@ -3473,7 +3483,7 @@ List<Expression> decreases, ref Attributes decAttrs, ref Attributes modAttrs, st
 		} else if (StartOf(9)) {
 			Expression(out ee, true, true);
 			e = ee; 
-		} else SynErr(225);
+		} else SynErr(226);
 	}
 
 	void AlternativeBlockCase(bool allowExistentialGuards, out GuardedAlternative alt) {
@@ -3488,13 +3498,13 @@ List<Expression> decreases, ref Attributes decAttrs, ref Attributes modAttrs, st
 			isExistentialGuard = true; 
 		} else if (StartOf(9)) {
 			Expression(out e, true, false);
-		} else SynErr(226);
+		} else SynErr(227);
 		Expect(31);
 		body = new List<Statement>(); 
-		while (!(StartOf(30))) {SynErr(227); Get();}
+		while (!(StartOf(30))) {SynErr(228); Get();}
 		while (IsNotEndOfCase()) {
 			Stmt(body);
-			while (!(StartOf(30))) {SynErr(228); Get();}
+			while (!(StartOf(30))) {SynErr(229); Get();}
 		}
 		alt = new GuardedAlternative(x, isExistentialGuard, e, body); 
 	}
@@ -3503,9 +3513,9 @@ List<Expression> decreases, ref Attributes decAttrs, ref Attributes modAttrs, st
 		Expression e; FrameExpression fe;
 		bool isFree = false; Attributes attrs = null;
 		
-		if (la.kind == 40 || la.kind == 97) {
-			while (!(la.kind == 0 || la.kind == 40 || la.kind == 97)) {SynErr(229); Get();}
-			if (la.kind == 97) {
+		if (la.kind == 40 || la.kind == 98) {
+			while (!(la.kind == 0 || la.kind == 40 || la.kind == 98)) {SynErr(230); Get();}
+			if (la.kind == 98) {
 				Get();
 				isFree = true; errors.Deprecated(t, "the 'free' keyword is soon to be deprecated"); 
 			}
@@ -3517,7 +3527,7 @@ List<Expression> decreases, ref Attributes decAttrs, ref Attributes modAttrs, st
 			invariants.Add(new MaybeFreeExpression(e, isFree, attrs)); 
 			OldSemi();
 		} else if (la.kind == 39) {
-			while (!(la.kind == 0 || la.kind == 39)) {SynErr(230); Get();}
+			while (!(la.kind == 0 || la.kind == 39)) {SynErr(231); Get();}
 			Get();
 			while (IsAttribute()) {
 				Attribute(ref decAttrs);
@@ -3525,7 +3535,7 @@ List<Expression> decreases, ref Attributes decAttrs, ref Attributes modAttrs, st
 			DecreasesList(decreases, true, true);
 			OldSemi();
 		} else if (la.kind == 47) {
-			while (!(la.kind == 0 || la.kind == 47)) {SynErr(231); Get();}
+			while (!(la.kind == 0 || la.kind == 47)) {SynErr(232); Get();}
 			Get();
 			mod = mod ?? new List<FrameExpression>(); 
 			while (IsAttribute()) {
@@ -3539,7 +3549,7 @@ List<Expression> decreases, ref Attributes decAttrs, ref Attributes modAttrs, st
 				mod.Add(fe); 
 			}
 			OldSemi();
-		} else SynErr(232);
+		} else SynErr(233);
 	}
 
 	void CaseStatement(out MatchCaseStmt/*!*/ c) {
@@ -3578,12 +3588,12 @@ List<Expression> decreases, ref Attributes decAttrs, ref Attributes modAttrs, st
 				arguments.Add(pat); 
 			}
 			Expect(55);
-		} else SynErr(233);
+		} else SynErr(234);
 		Expect(31);
-		while (!(StartOf(30))) {SynErr(234); Get();}
+		while (!(StartOf(30))) {SynErr(235); Get();}
 		while (IsNotEndOfCase()) {
 			Stmt(body);
-			while (!(StartOf(30))) {SynErr(235); Get();}
+			while (!(StartOf(30))) {SynErr(236); Get();}
 		}
 		c = new MatchCaseStmt(x, name, arguments, body); 
 	}
@@ -3619,7 +3629,7 @@ List<Expression> decreases, ref Attributes decAttrs, ref Attributes modAttrs, st
 		case 58: {
 			Get();
 			x = t;  binOp = BinaryExpr.Opcode.Eq; 
-			if (la.kind == 113) {
+			if (la.kind == 114) {
 				Get();
 				Expect(52);
 				Expression(out k, true, true);
@@ -3637,12 +3647,12 @@ List<Expression> decreases, ref Attributes decAttrs, ref Attributes modAttrs, st
 			x = t;  binOp = BinaryExpr.Opcode.Gt; 
 			break;
 		}
-		case 114: {
+		case 115: {
 			Get();
 			x = t;  binOp = BinaryExpr.Opcode.Le; 
 			break;
 		}
-		case 115: {
+		case 116: {
 			Get();
 			x = t;  binOp = BinaryExpr.Opcode.Ge; 
 			break;
@@ -3657,32 +3667,32 @@ List<Expression> decreases, ref Attributes decAttrs, ref Attributes modAttrs, st
 			x = t;  binOp = BinaryExpr.Opcode.Neq; 
 			break;
 		}
-		case 116: {
+		case 117: {
 			Get();
 			x = t;  binOp = BinaryExpr.Opcode.Le; 
 			break;
 		}
-		case 117: {
+		case 118: {
 			Get();
 			x = t;  binOp = BinaryExpr.Opcode.Ge; 
 			break;
 		}
-		case 118: case 119: {
+		case 119: case 120: {
 			EquivOp();
 			x = t;  binOp = BinaryExpr.Opcode.Iff; 
 			break;
 		}
-		case 120: case 121: {
+		case 121: case 122: {
 			ImpliesOp();
 			x = t;  binOp = BinaryExpr.Opcode.Imp; 
 			break;
 		}
-		case 122: case 123: {
+		case 123: case 124: {
 			ExpliesOp();
 			x = t;  binOp = BinaryExpr.Opcode.Exp; 
 			break;
 		}
-		default: SynErr(236); break;
+		default: SynErr(237); break;
 		}
 		if (k == null) {
 		 op = new Microsoft.Dafny.CalcStmt.BinaryCalcOp(binOp);
@@ -3693,67 +3703,67 @@ List<Expression> decreases, ref Attributes decAttrs, ref Attributes modAttrs, st
 	}
 
 	void EquivOp() {
-		if (la.kind == 118) {
+		if (la.kind == 119) {
 			Get();
-		} else if (la.kind == 119) {
-			Get();
-		} else SynErr(237);
-	}
-
-	void ImpliesOp() {
-		if (la.kind == 120) {
-			Get();
-		} else if (la.kind == 121) {
+		} else if (la.kind == 120) {
 			Get();
 		} else SynErr(238);
 	}
 
-	void ExpliesOp() {
-		if (la.kind == 122) {
+	void ImpliesOp() {
+		if (la.kind == 121) {
 			Get();
-		} else if (la.kind == 123) {
+		} else if (la.kind == 122) {
 			Get();
 		} else SynErr(239);
 	}
 
-	void AndOp() {
-		if (la.kind == 124) {
+	void ExpliesOp() {
+		if (la.kind == 123) {
 			Get();
-		} else if (la.kind == 125) {
+		} else if (la.kind == 124) {
 			Get();
 		} else SynErr(240);
 	}
 
-	void OrOp() {
-		if (la.kind == 126) {
+	void AndOp() {
+		if (la.kind == 125) {
 			Get();
-		} else if (la.kind == 127) {
+		} else if (la.kind == 126) {
 			Get();
 		} else SynErr(241);
 	}
 
-	void NegOp() {
-		if (la.kind == 128) {
+	void OrOp() {
+		if (la.kind == 127) {
 			Get();
-		} else if (la.kind == 129) {
+		} else if (la.kind == 128) {
 			Get();
 		} else SynErr(242);
 	}
 
-	void Forall() {
-		if (la.kind == 110) {
+	void NegOp() {
+		if (la.kind == 129) {
 			Get();
 		} else if (la.kind == 130) {
 			Get();
 		} else SynErr(243);
 	}
 
-	void Exists() {
-		if (la.kind == 131) {
+	void Forall() {
+		if (la.kind == 111) {
 			Get();
-		} else if (la.kind == 132) {
+		} else if (la.kind == 131) {
 			Get();
 		} else SynErr(244);
+	}
+
+	void Exists() {
+		if (la.kind == 132) {
+			Get();
+		} else if (la.kind == 133) {
+			Get();
+		} else SynErr(245);
 	}
 
 	void QSep() {
@@ -3761,7 +3771,7 @@ List<Expression> decreases, ref Attributes decAttrs, ref Attributes modAttrs, st
 			Get();
 		} else if (la.kind == 27) {
 			Get();
-		} else SynErr(245);
+		} else SynErr(246);
 	}
 
 	void EquivExpression(out Expression e0, bool allowSemi, bool allowLambda, bool allowBitwiseOps) {
@@ -3779,12 +3789,12 @@ List<Expression> decreases, ref Attributes decAttrs, ref Attributes modAttrs, st
 		Contract.Ensures(Contract.ValueAtReturn(out e0) != null); IToken/*!*/ x;  Expression/*!*/ e1; 
 		LogicalExpression(out e0, allowSemi, allowLambda, allowBitwiseOps);
 		if (IsImpliesOp() || IsExpliesOp()) {
-			if (la.kind == 120 || la.kind == 121) {
+			if (la.kind == 121 || la.kind == 122) {
 				ImpliesOp();
 				x = t; 
 				ImpliesExpression(out e1, allowSemi, allowLambda, allowBitwiseOps);
 				e0 = new BinaryExpr(x, BinaryExpr.Opcode.Imp, e0, e1); 
-			} else if (la.kind == 122 || la.kind == 123) {
+			} else if (la.kind == 123 || la.kind == 124) {
 				ExpliesOp();
 				x = t; 
 				LogicalExpression(out e1, allowSemi, allowLambda, allowBitwiseOps);
@@ -3796,7 +3806,7 @@ List<Expression> decreases, ref Attributes decAttrs, ref Attributes modAttrs, st
 					e0 = new BinaryExpr(x, BinaryExpr.Opcode.Exp, e1, e0); 
 					
 				}
-			} else SynErr(246);
+			} else SynErr(247);
 		}
 	}
 
@@ -3805,7 +3815,7 @@ List<Expression> decreases, ref Attributes decAttrs, ref Attributes modAttrs, st
 		Expression first;
 		e0 = dummyExpr; /* mute the warning */
 		
-		if (la.kind == 124 || la.kind == 125) {
+		if (la.kind == 125 || la.kind == 126) {
 			AndOp();
 			x = t; 
 			RelationalExpression(out e0, allowSemi, allowLambda, allowBitwiseOps);
@@ -3822,7 +3832,7 @@ List<Expression> decreases, ref Attributes decAttrs, ref Attributes modAttrs, st
 			 e0 = new BinaryExpr(x, BinaryExpr.Opcode.And, new LiteralExpr(x, true), e0);
 			}
 			
-		} else if (la.kind == 126 || la.kind == 127) {
+		} else if (la.kind == 127 || la.kind == 128) {
 			OrOp();
 			x = t; 
 			RelationalExpression(out e0, allowSemi, allowLambda, allowBitwiseOps);
@@ -3842,7 +3852,7 @@ List<Expression> decreases, ref Attributes decAttrs, ref Attributes modAttrs, st
 		} else if (StartOf(31)) {
 			RelationalExpression(out e0, allowSemi, allowLambda, allowBitwiseOps);
 			if (IsAndOp() || IsOrOp()) {
-				if (la.kind == 124 || la.kind == 125) {
+				if (la.kind == 125 || la.kind == 126) {
 					AndOp();
 					x = t; 
 					RelationalExpression(out e1, allowSemi, allowLambda, allowBitwiseOps);
@@ -3853,7 +3863,7 @@ List<Expression> decreases, ref Attributes decAttrs, ref Attributes modAttrs, st
 						RelationalExpression(out e1, allowSemi, allowLambda, allowBitwiseOps);
 						e0 = new BinaryExpr(x, BinaryExpr.Opcode.And, e0, e1); 
 					}
-				} else if (la.kind == 126 || la.kind == 127) {
+				} else if (la.kind == 127 || la.kind == 128) {
 					OrOp();
 					x = t; 
 					RelationalExpression(out e1, allowSemi, allowLambda, allowBitwiseOps);
@@ -3864,9 +3874,9 @@ List<Expression> decreases, ref Attributes decAttrs, ref Attributes modAttrs, st
 						RelationalExpression(out e1, allowSemi, allowLambda, allowBitwiseOps);
 						e0 = new BinaryExpr(x, BinaryExpr.Opcode.Or, e0, e1); 
 					}
-				} else SynErr(247);
+				} else SynErr(248);
 			}
-		} else SynErr(248);
+		} else SynErr(249);
 	}
 
 	void ImpliesExpression(out Expression e0, bool allowSemi, bool allowLambda, bool allowBitwiseOps) {
@@ -3986,7 +3996,7 @@ List<Expression> decreases, ref Attributes decAttrs, ref Attributes modAttrs, st
 				x = t;  op = BinaryExpr.Opcode.RightShift; 
 				Expect(57);
 				x.val = "<<";  Contract.Assert(t.pos == x.pos + 1); 
-			} else SynErr(249);
+			} else SynErr(250);
 			Term(out e1, allowSemi, allowLambda, allowBitwiseOps);
 			e0 = new BinaryExpr(x, op, e0, e1); 
 		}
@@ -4002,7 +4012,7 @@ List<Expression> decreases, ref Attributes decAttrs, ref Attributes modAttrs, st
 		case 58: {
 			Get();
 			x = t;  op = BinaryExpr.Opcode.Eq; 
-			if (la.kind == 113) {
+			if (la.kind == 114) {
 				Get();
 				Expect(52);
 				Expression(out k, true, true);
@@ -4020,12 +4030,12 @@ List<Expression> decreases, ref Attributes decAttrs, ref Attributes modAttrs, st
 			x = t;  op = BinaryExpr.Opcode.Gt; 
 			break;
 		}
-		case 114: {
+		case 115: {
 			Get();
 			x = t;  op = BinaryExpr.Opcode.Le; 
 			break;
 		}
-		case 115: {
+		case 116: {
 			Get();
 			x = t;  op = BinaryExpr.Opcode.Ge; 
 			break;
@@ -4033,7 +4043,7 @@ List<Expression> decreases, ref Attributes decAttrs, ref Attributes modAttrs, st
 		case 59: {
 			Get();
 			x = t;  op = BinaryExpr.Opcode.Neq; 
-			if (la.kind == 113) {
+			if (la.kind == 114) {
 				Get();
 				Expect(52);
 				Expression(out k, true, true);
@@ -4041,7 +4051,7 @@ List<Expression> decreases, ref Attributes decAttrs, ref Attributes modAttrs, st
 			}
 			break;
 		}
-		case 133: {
+		case 134: {
 			Get();
 			x = t;  op = BinaryExpr.Opcode.In; 
 			break;
@@ -4051,11 +4061,11 @@ List<Expression> decreases, ref Attributes decAttrs, ref Attributes modAttrs, st
 			x = t;  op = BinaryExpr.Opcode.NotIn; 
 			break;
 		}
-		case 128: {
+		case 129: {
 			Get();
 			x = t;  y = Token.NoToken; 
 			if (la.val == "!") {
-				Expect(128);
+				Expect(129);
 				y = t; 
 			}
 			if (y == Token.NoToken) {
@@ -4074,17 +4084,17 @@ List<Expression> decreases, ref Attributes decAttrs, ref Attributes modAttrs, st
 			x = t;  op = BinaryExpr.Opcode.Neq; 
 			break;
 		}
-		case 116: {
+		case 117: {
 			Get();
 			x = t;  op = BinaryExpr.Opcode.Le; 
 			break;
 		}
-		case 117: {
+		case 118: {
 			Get();
 			x = t;  op = BinaryExpr.Opcode.Ge; 
 			break;
 		}
-		default: SynErr(250); break;
+		default: SynErr(251); break;
 		}
 	}
 
@@ -4110,27 +4120,27 @@ List<Expression> decreases, ref Attributes decAttrs, ref Attributes modAttrs, st
 
 	void AddOp(out IToken x, out BinaryExpr.Opcode op) {
 		Contract.Ensures(Contract.ValueAtReturn(out x) != null); x = Token.NoToken;  op=BinaryExpr.Opcode.Add/*(dummy)*/; 
-		if (la.kind == 134) {
+		if (la.kind == 135) {
 			Get();
 			x = t;  op = BinaryExpr.Opcode.Add; 
-		} else if (la.kind == 135) {
+		} else if (la.kind == 136) {
 			Get();
 			x = t;  op = BinaryExpr.Opcode.Sub; 
-		} else SynErr(251);
+		} else SynErr(252);
 	}
 
 	void BitvectorFactor(out Expression e0, bool allowSemi, bool allowLambda, bool allowBitwiseOps) {
 		Contract.Ensures(Contract.ValueAtReturn(out e0) != null); IToken/*!*/ x;  Expression/*!*/ e1;  BinaryExpr.Opcode op; 
 		AsExpression(out e0, allowSemi, allowLambda, allowBitwiseOps);
 		if (allowBitwiseOps && IsBitwiseOp()) {
-			if (la.kind == 138) {
+			if (la.kind == 139) {
 				op = BinaryExpr.Opcode.BitwiseAnd; 
 				Get();
 				x = t; 
 				AsExpression(out e1, allowSemi, allowLambda, allowBitwiseOps);
 				e0 = new BinaryExpr(x, op, e0, e1); 
 				while (IsBitwiseAndOp()) {
-					Expect(138);
+					Expect(139);
 					x = t; 
 					AsExpression(out e1, allowSemi, allowLambda, allowBitwiseOps);
 					e0 = new BinaryExpr(x, op, e0, e1); 
@@ -4147,19 +4157,19 @@ List<Expression> decreases, ref Attributes decAttrs, ref Attributes modAttrs, st
 					AsExpression(out e1, allowSemi, allowLambda, allowBitwiseOps);
 					e0 = new BinaryExpr(x, op, e0, e1); 
 				}
-			} else if (la.kind == 139) {
+			} else if (la.kind == 140) {
 				op = BinaryExpr.Opcode.BitwiseXor; 
 				Get();
 				x = t; 
 				AsExpression(out e1, allowSemi, allowLambda, allowBitwiseOps);
 				e0 = new BinaryExpr(x, op, e0, e1); 
 				while (IsBitwiseXorOp()) {
-					Expect(139);
+					Expect(140);
 					x = t; 
 					AsExpression(out e1, allowSemi, allowLambda, allowBitwiseOps);
 					e0 = new BinaryExpr(x, op, e0, e1); 
 				}
-			} else SynErr(252);
+			} else SynErr(253);
 		}
 	}
 
@@ -4168,13 +4178,13 @@ List<Expression> decreases, ref Attributes decAttrs, ref Attributes modAttrs, st
 		if (la.kind == 61) {
 			Get();
 			x = t;  op = BinaryExpr.Opcode.Mul; 
-		} else if (la.kind == 136) {
-			Get();
-			x = t;  op = BinaryExpr.Opcode.Div; 
 		} else if (la.kind == 137) {
 			Get();
+			x = t;  op = BinaryExpr.Opcode.Div; 
+		} else if (la.kind == 138) {
+			Get();
 			x = t;  op = BinaryExpr.Opcode.Mod; 
-		} else SynErr(253);
+		} else SynErr(254);
 	}
 
 	void AsExpression(out Expression e, bool allowSemi, bool allowLambda, bool allowBitwiseOps) {
@@ -4190,12 +4200,12 @@ List<Expression> decreases, ref Attributes decAttrs, ref Attributes modAttrs, st
 
 	void UnaryExpression(out Expression e, bool allowSemi, bool allowLambda, bool allowBitwiseOps) {
 		Contract.Ensures(Contract.ValueAtReturn(out e) != null); IToken/*!*/ x;  e = dummyExpr; 
-		if (la.kind == 135) {
+		if (la.kind == 136) {
 			Get();
 			x = t; 
 			UnaryExpression(out e, allowSemi, allowLambda, allowBitwiseOps);
 			e = new NegationExpression(x, e); 
-		} else if (la.kind == 128 || la.kind == 129) {
+		} else if (la.kind == 129 || la.kind == 130) {
 			NegOp();
 			x = t; 
 			UnaryExpression(out e, allowSemi, allowLambda, allowBitwiseOps);
@@ -4245,7 +4255,7 @@ List<Expression> decreases, ref Attributes decAttrs, ref Attributes modAttrs, st
 			while (IsSuffix()) {
 				Suffix(ref e);
 			}
-		} else SynErr(254);
+		} else SynErr(255);
 	}
 
 	void MapDisplayExpr(IToken/*!*/ mapToken, bool finite, out Expression e) {
@@ -4296,23 +4306,23 @@ List<Expression> decreases, ref Attributes decAttrs, ref Attributes modAttrs, st
 				if (IsGenericInstantiation(true)) {
 					typeArgs = new List<Type>(); 
 					GenericInstantiation(typeArgs);
-				} else if (la.kind == 113) {
+				} else if (la.kind == 114) {
 					HashCall(id, out openParen, out typeArgs, out args);
 				} else if (StartOf(33)) {
-				} else SynErr(255);
+				} else SynErr(256);
 				e = new ExprDotName(id, e, id.val, typeArgs);
 				if (openParen != null) {
 				 e = new ApplySuffix(openParen, e, args);
 				}
 				
-			} else SynErr(256);
+			} else SynErr(257);
 		} else if (la.kind == 52) {
 			Get();
 			x = t; 
 			if (StartOf(9)) {
 				Expression(out ee, true, true);
 				e0 = ee; 
-				if (la.kind == 148) {
+				if (la.kind == 149) {
 					Get();
 					anyDots = true; 
 					if (StartOf(9)) {
@@ -4353,15 +4363,15 @@ List<Expression> decreases, ref Attributes decAttrs, ref Attributes modAttrs, st
 						multipleIndices.Add(ee);
 						
 					}
-				} else SynErr(257);
-			} else if (la.kind == 148) {
+				} else SynErr(258);
+			} else if (la.kind == 149) {
 				Get();
 				anyDots = true; 
 				if (StartOf(9)) {
 					Expression(out ee, true, true);
 					e1 = ee; 
 				}
-			} else SynErr(258);
+			} else SynErr(259);
 			if (multipleIndices != null) {
 			 e = new MultiSelectExpr(x, e, multipleIndices);
 			 // make sure an array class with this dimensionality exists
@@ -4405,7 +4415,7 @@ List<Expression> decreases, ref Attributes decAttrs, ref Attributes modAttrs, st
 			}
 			Expect(55);
 			e = new ApplySuffix(openParen, e, args); 
-		} else SynErr(259);
+		} else SynErr(260);
 	}
 
 	void ISetDisplayExpr(IToken/*!*/ setToken, bool finite, out Expression e) {
@@ -4447,7 +4457,7 @@ List<Expression> decreases, ref Attributes decAttrs, ref Attributes modAttrs, st
 				}
 			}
 			Expect(55);
-		} else SynErr(260);
+		} else SynErr(261);
 		while (la.kind == 48 || la.kind == 49) {
 			if (la.kind == 48) {
 				Get();
@@ -4479,7 +4489,7 @@ List<Expression> decreases, ref Attributes decAttrs, ref Attributes modAttrs, st
 		e = dummyExpr;
 		
 		switch (la.kind) {
-		case 104: {
+		case 105: {
 			Get();
 			x = t; 
 			if (IsExistentialGuard()) {
@@ -4487,7 +4497,7 @@ List<Expression> decreases, ref Attributes decAttrs, ref Attributes modAttrs, st
 				isExistentialGuard = true; 
 			} else if (StartOf(9)) {
 				Expression(out e, true, true);
-			} else SynErr(261);
+			} else SynErr(262);
 			Expect(36);
 			Expression(out e0, true, true, true);
 			Expect(37);
@@ -4504,11 +4514,11 @@ List<Expression> decreases, ref Attributes decAttrs, ref Attributes modAttrs, st
 			
 			break;
 		}
-		case 106: {
+		case 107: {
 			MatchExpression(out e, allowSemi, allowLambda, allowBitwiseOps);
 			break;
 		}
-		case 110: case 130: case 131: case 132: {
+		case 111: case 131: case 132: case 133: {
 			QuantifierGuts(out e, allowSemi, allowLambda);
 			break;
 		}
@@ -4524,7 +4534,7 @@ List<Expression> decreases, ref Attributes decAttrs, ref Attributes modAttrs, st
 			SetComprehensionExpr(x, false, out e, allowSemi, allowLambda, true);
 			break;
 		}
-		case 33: case 34: case 107: {
+		case 33: case 34: case 108: {
 			StmtInExpr(out s);
 			Expression(out e, allowSemi, allowLambda, allowBitwiseOps);
 			e = new StmtExpr(s.Tok, s, e); 
@@ -4552,11 +4562,11 @@ List<Expression> decreases, ref Attributes decAttrs, ref Attributes modAttrs, st
 			e = new RevealExpr(e.tok, e); 
 			break;
 		}
-		case 100: {
+		case 101: {
 			NamedExpr(out e, allowSemi, allowLambda, allowBitwiseOps);
 			break;
 		}
-		default: SynErr(262); break;
+		default: SynErr(263); break;
 		}
 	}
 
@@ -4568,10 +4578,10 @@ List<Expression> decreases, ref Attributes decAttrs, ref Attributes modAttrs, st
 		if (IsGenericInstantiation(true)) {
 			typeArgs = new List<Type>(); 
 			GenericInstantiation(typeArgs);
-		} else if (la.kind == 113) {
+		} else if (la.kind == 114) {
 			HashCall(id, out openParen, out typeArgs, out args);
 		} else if (StartOf(33)) {
-		} else SynErr(263);
+		} else SynErr(264);
 		e = new NameSegment(id, id.val, typeArgs);
 		if (openParen != null) {
 		 e = new ApplySuffix(openParen, e, args);
@@ -4600,7 +4610,7 @@ List<Expression> decreases, ref Attributes decAttrs, ref Attributes modAttrs, st
 			}
 			e = new SeqDisplayExpr(x, elements); 
 			Expect(53);
-		} else SynErr(264);
+		} else SynErr(265);
 	}
 
 	void MultiSetExpr(out Expression e) {
@@ -4624,7 +4634,7 @@ List<Expression> decreases, ref Attributes decAttrs, ref Attributes modAttrs, st
 			Expression(out e, true, true);
 			e = new MultiSetFormingExpr(x, e); 
 			Expect(55);
-		} else SynErr(265);
+		} else SynErr(266);
 	}
 
 	void ConstAtomExpression(out Expression e, bool allowSemi, bool allowLambda) {
@@ -4633,17 +4643,17 @@ List<Expression> decreases, ref Attributes decAttrs, ref Attributes modAttrs, st
 		e = dummyExpr;  Type toType = null;
 		
 		switch (la.kind) {
-		case 140: {
+		case 141: {
 			Get();
 			e = new LiteralExpr(t, false); 
 			break;
 		}
-		case 141: {
+		case 142: {
 			Get();
 			e = new LiteralExpr(t, true); 
 			break;
 		}
-		case 142: {
+		case 143: {
 			Get();
 			e = new LiteralExpr(t); 
 			break;
@@ -4671,18 +4681,9 @@ List<Expression> decreases, ref Attributes decAttrs, ref Attributes modAttrs, st
 			
 			break;
 		}
-		case 143: {
-			Get();
-			e = new ThisExpr(t); 
-			break;
-		}
 		case 144: {
 			Get();
-			x = t; 
-			Expect(54);
-			Expression(out e, true, true);
-			Expect(55);
-			e = new UnaryOpExpr(x, UnaryOpExpr.Opcode.Fresh, e); 
+			e = new ThisExpr(t); 
 			break;
 		}
 		case 145: {
@@ -4691,10 +4692,19 @@ List<Expression> decreases, ref Attributes decAttrs, ref Attributes modAttrs, st
 			Expect(54);
 			Expression(out e, true, true);
 			Expect(55);
-			e = new UnaryOpExpr(x, UnaryOpExpr.Opcode.Allocated, e); 
+			e = new UnaryOpExpr(x, UnaryOpExpr.Opcode.Fresh, e); 
 			break;
 		}
 		case 146: {
+			Get();
+			x = t; 
+			Expect(54);
+			Expression(out e, true, true);
+			Expect(55);
+			e = new UnaryOpExpr(x, UnaryOpExpr.Opcode.Allocated, e); 
+			break;
+		}
+		case 147: {
 			Get();
 			x = t; FrameExpression fe; var mod = new List<FrameExpression>(); 
 			Expect(54);
@@ -4709,7 +4719,7 @@ List<Expression> decreases, ref Attributes decAttrs, ref Attributes modAttrs, st
 			e = new UnchangedExpr(x, mod); 
 			break;
 		}
-		case 147: {
+		case 148: {
 			Get();
 			x = t; 
 			Expect(54);
@@ -4745,7 +4755,7 @@ List<Expression> decreases, ref Attributes decAttrs, ref Attributes modAttrs, st
 			ParensExpression(out e, allowSemi, allowLambda);
 			break;
 		}
-		default: SynErr(266); break;
+		default: SynErr(267); break;
 		}
 	}
 
@@ -4774,7 +4784,7 @@ List<Expression> decreases, ref Attributes decAttrs, ref Attributes modAttrs, st
 			 n = BigInteger.Zero;
 			}
 			
-		} else SynErr(267);
+		} else SynErr(268);
 	}
 
 	void Dec(out Basetypes.BigDec d) {
@@ -4818,7 +4828,7 @@ List<Expression> decreases, ref Attributes decAttrs, ref Attributes modAttrs, st
 		} else if (la.kind == 32) {
 			Get();
 			oneShot = true; 
-		} else SynErr(268);
+		} else SynErr(269);
 	}
 
 	void MapLiteralExpressions(out List<ExpressionPair> elements) {
@@ -4865,7 +4875,7 @@ List<Expression> decreases, ref Attributes decAttrs, ref Attributes modAttrs, st
 		List<MatchCaseExpr/*!*/> cases = new List<MatchCaseExpr/*!*/>();
 		bool usesOptionalBraces = false;
 		
-		Expect(106);
+		Expect(107);
 		x = t; 
 		Expression(out e, allowSemi, allowLambda, allowBitwiseOps);
 		if (la.kind == _lbrace) {
@@ -4881,7 +4891,7 @@ List<Expression> decreases, ref Attributes decAttrs, ref Attributes modAttrs, st
 				CaseExpression(out c, allowSemi, allowLambda, allowBitwiseOps);
 				cases.Add(c); 
 			}
-		} else SynErr(269);
+		} else SynErr(270);
 		e = new MatchExpr(x, e, cases, usesOptionalBraces); 
 	}
 
@@ -4893,13 +4903,13 @@ List<Expression> decreases, ref Attributes decAttrs, ref Attributes modAttrs, st
 		Expression range;
 		Expression/*!*/ body;
 		
-		if (la.kind == 110 || la.kind == 130) {
+		if (la.kind == 111 || la.kind == 131) {
 			Forall();
 			x = t;  univ = true; 
-		} else if (la.kind == 131 || la.kind == 132) {
+		} else if (la.kind == 132 || la.kind == 133) {
 			Exists();
 			x = t; 
-		} else SynErr(270);
+		} else SynErr(271);
 		QuantifierDomain(out bvars, out attrs, out range);
 		QSep();
 		Expression(out body, allowSemi, allowLambda);
@@ -4942,13 +4952,13 @@ List<Expression> decreases, ref Attributes decAttrs, ref Attributes modAttrs, st
 
 	void StmtInExpr(out Statement s) {
 		s = dummyStmt; 
-		if (la.kind == 107) {
+		if (la.kind == 108) {
 			AssertStmt(out s);
 		} else if (la.kind == 33) {
 			AssumeStmt(out s);
 		} else if (la.kind == 34) {
 			CalcStmt(out s);
-		} else SynErr(271);
+		} else SynErr(272);
 	}
 
 	void LetExpr(out Expression e, bool allowSemi, bool allowLambda, bool allowBitwiseOps) {
@@ -4992,7 +5002,7 @@ List<Expression> decreases, ref Attributes decAttrs, ref Attributes modAttrs, st
 			 }
 			}
 			
-		} else SynErr(272);
+		} else SynErr(273);
 		Expression(out e, false, true);
 		letRHSs.Add(e); 
 		while (la.kind == 23) {
@@ -5010,7 +5020,7 @@ List<Expression> decreases, ref Attributes decAttrs, ref Attributes modAttrs, st
 		e = dummyExpr;
 		Expression expr;
 		
-		Expect(100);
+		Expect(101);
 		x = t; 
 		NoUSIdent(out d);
 		Expect(22);
@@ -5054,7 +5064,7 @@ List<Expression> decreases, ref Attributes decAttrs, ref Attributes modAttrs, st
 				arguments.Add(pat); 
 			}
 			Expect(55);
-		} else SynErr(273);
+		} else SynErr(274);
 		Expect(31);
 		Expression(out body, allowSemi, allowLambda, allowBitwiseOps);
 		c = new MatchCaseExpr(x, name, arguments, body); 
@@ -5062,7 +5072,7 @@ List<Expression> decreases, ref Attributes decAttrs, ref Attributes modAttrs, st
 
 	void HashCall(IToken id, out IToken openParen, out List<Type> typeArgs, out List<Expression> args) {
 		Expression k; args = new List<Expression>(); typeArgs = null; 
-		Expect(113);
+		Expect(114);
 		id.val = id.val + "#"; 
 		if (la.kind == 56) {
 			typeArgs = new List<Type>(); 
@@ -5088,7 +5098,7 @@ List<Expression> decreases, ref Attributes decAttrs, ref Attributes modAttrs, st
 		} else if (la.kind == 2) {
 			Get();
 			id = t; 
-		} else SynErr(274);
+		} else SynErr(275);
 		Expect(86);
 		Expression(out e, true, true);
 	}
@@ -5105,41 +5115,41 @@ List<Expression> decreases, ref Attributes decAttrs, ref Attributes modAttrs, st
   }
 
   static readonly bool[,] set = {
-		{_T,_T,_T,_T, _T,_x,_x,_x, _x,_T,_x,_T, _x,_x,_x,_x, _x,_x,_x,_x, _T,_T,_x,_x, _T,_x,_x,_x, _x,_x,_T,_x, _x,_T,_T,_T, _x,_x,_x,_T, _T,_x,_x,_T, _T,_T,_x,_T, _T,_T,_T,_T, _x,_x,_T,_x, _x,_x,_x,_x, _x,_x,_x,_T, _T,_x,_x,_T, _x,_x,_x,_x, _x,_x,_x,_x, _x,_x,_x,_x, _T,_T,_T,_T, _T,_T,_x,_x, _x,_x,_T,_x, _x,_T,_T,_T, _T,_T,_T,_T, _T,_T,_x,_T, _T,_T,_T,_T, _x,_T,_T,_T, _T,_x,_x,_x, _x,_x,_x,_x, _x,_x,_x,_x, _x,_x,_x,_x, _x,_x,_x,_x, _x,_x,_x,_x, _x,_x,_x,_x, _T,_T,_T,_T, _T,_T,_T,_T, _x,_x,_x},
-		{_x,_x,_x,_x, _x,_x,_x,_x, _x,_x,_x,_x, _x,_x,_x,_x, _x,_x,_x,_x, _x,_x,_x,_x, _x,_x,_x,_x, _x,_x,_x,_x, _x,_x,_x,_x, _x,_x,_x,_x, _x,_T,_T,_T, _T,_T,_T,_x, _x,_x,_x,_x, _x,_x,_x,_x, _x,_x,_x,_x, _x,_x,_x,_x, _x,_x,_T,_T, _T,_T,_T,_T, _x,_T,_x,_x, _T,_x,_x,_x, _T,_T,_T,_T, _T,_T,_x,_T, _T,_x,_T,_x, _x,_T,_T,_T, _T,_x,_x,_x, _x,_x,_x,_x, _x,_x,_x,_x, _x,_x,_x,_x, _x,_x,_x,_x, _x,_x,_x,_x, _x,_x,_x,_x, _x,_x,_x,_x, _x,_x,_x,_x, _x,_x,_x,_x, _x,_x,_x,_x, _x,_x,_x,_x, _x,_x,_x,_x, _x,_x,_x},
-		{_x,_x,_x,_x, _x,_x,_x,_x, _x,_x,_x,_x, _x,_x,_x,_x, _x,_x,_x,_x, _x,_x,_x,_x, _x,_x,_x,_x, _x,_x,_x,_x, _x,_x,_x,_x, _x,_x,_x,_x, _x,_x,_x,_x, _x,_x,_x,_x, _x,_x,_x,_x, _x,_x,_x,_x, _x,_x,_x,_x, _x,_x,_x,_x, _x,_x,_T,_T, _T,_T,_T,_x, _x,_x,_x,_x, _x,_x,_x,_x, _x,_x,_x,_x, _x,_x,_x,_x, _x,_x,_x,_x, _x,_x,_x,_x, _x,_x,_x,_x, _x,_x,_x,_x, _x,_x,_x,_x, _x,_x,_x,_x, _x,_x,_x,_x, _x,_x,_x,_x, _x,_x,_x,_x, _x,_x,_x,_x, _x,_x,_x,_x, _x,_x,_x,_x, _x,_x,_x,_x, _x,_x,_x,_x, _x,_x,_x,_x, _x,_x,_x},
-		{_T,_x,_x,_x, _x,_x,_x,_x, _x,_x,_x,_x, _x,_x,_x,_x, _x,_x,_x,_x, _x,_x,_x,_x, _x,_x,_x,_x, _T,_T,_T,_x, _x,_x,_x,_x, _x,_x,_x,_x, _x,_T,_T,_T, _T,_T,_T,_x, _x,_x,_x,_T, _x,_x,_x,_x, _x,_x,_x,_x, _x,_x,_x,_x, _x,_x,_T,_T, _T,_T,_T,_T, _x,_T,_x,_x, _T,_x,_x,_x, _T,_T,_T,_T, _T,_T,_x,_T, _T,_x,_T,_x, _x,_T,_T,_T, _T,_x,_x,_x, _x,_x,_x,_x, _x,_x,_x,_x, _x,_x,_x,_x, _x,_x,_x,_x, _x,_x,_x,_x, _x,_x,_x,_x, _x,_x,_x,_x, _x,_x,_x,_x, _x,_x,_x,_x, _x,_x,_x,_x, _x,_x,_x,_x, _x,_x,_x,_x, _x,_x,_x},
-		{_x,_T,_T,_x, _T,_x,_x,_x, _x,_x,_x,_x, _x,_x,_x,_x, _x,_x,_x,_x, _x,_x,_x,_x, _x,_x,_x,_x, _x,_x,_x,_x, _x,_x,_x,_x, _x,_x,_x,_x, _x,_x,_x,_x, _x,_x,_x,_x, _T,_T,_x,_x, _x,_x,_x,_x, _x,_x,_x,_x, _x,_x,_x,_x, _x,_x,_x,_x, _x,_x,_x,_x, _x,_x,_x,_x, _x,_x,_x,_x, _x,_x,_x,_x, _x,_x,_x,_x, _x,_x,_x,_x, _x,_x,_x,_x, _x,_x,_x,_x, _x,_x,_x,_x, _x,_x,_x,_x, _x,_x,_x,_x, _x,_x,_x,_x, _x,_x,_x,_x, _x,_x,_x,_x, _x,_x,_x,_x, _x,_x,_x,_x, _x,_x,_x,_x, _x,_x,_x,_x, _x,_x,_x,_x, _x,_x,_x,_x, _x,_x,_x},
-		{_x,_x,_x,_x, _x,_x,_x,_x, _x,_x,_x,_x, _x,_x,_x,_x, _x,_x,_x,_x, _x,_x,_x,_x, _x,_x,_x,_x, _x,_x,_x,_x, _x,_x,_x,_x, _x,_x,_x,_x, _x,_T,_T,_T, _T,_T,_T,_x, _x,_x,_x,_x, _x,_x,_x,_x, _x,_x,_x,_x, _x,_x,_x,_x, _x,_x,_T,_T, _T,_T,_T,_x, _x,_x,_x,_x, _x,_x,_x,_x, _x,_x,_x,_x, _T,_T,_x,_x, _x,_x,_x,_x, _x,_T,_T,_T, _T,_x,_x,_x, _x,_x,_x,_x, _x,_x,_x,_x, _x,_x,_x,_x, _x,_x,_x,_x, _x,_x,_x,_x, _x,_x,_x,_x, _x,_x,_x,_x, _x,_x,_x,_x, _x,_x,_x,_x, _x,_x,_x,_x, _x,_x,_x,_x, _x,_x,_x,_x, _x,_x,_x},
-		{_x,_T,_x,_x, _x,_T,_T,_T, _T,_T,_T,_T, _T,_T,_T,_T, _T,_T,_T,_T, _x,_x,_x,_x, _x,_x,_x,_x, _x,_x,_x,_x, _x,_x,_x,_x, _x,_x,_x,_x, _x,_x,_x,_x, _x,_x,_x,_x, _x,_x,_x,_x, _x,_x,_T,_x, _x,_x,_x,_x, _x,_x,_x,_x, _x,_x,_x,_x, _x,_x,_x,_x, _x,_x,_x,_x, _x,_x,_x,_x, _x,_x,_x,_x, _x,_x,_x,_x, _x,_x,_x,_x, _x,_x,_x,_x, _x,_x,_x,_x, _x,_x,_x,_x, _x,_x,_x,_x, _x,_x,_x,_x, _x,_x,_x,_x, _x,_x,_x,_x, _x,_x,_x,_x, _x,_x,_x,_x, _x,_x,_x,_x, _x,_x,_x,_x, _x,_x,_x,_x, _x,_x,_x,_x, _x,_x,_x,_x, _x,_x,_x},
-		{_x,_x,_x,_x, _x,_x,_x,_x, _x,_x,_x,_x, _x,_x,_x,_x, _x,_x,_x,_x, _x,_x,_x,_x, _x,_x,_x,_x, _x,_x,_x,_x, _x,_x,_x,_x, _x,_x,_x,_T, _x,_x,_x,_x, _x,_x,_x,_T, _T,_T,_x,_x, _x,_x,_x,_x, _x,_x,_x,_x, _x,_x,_x,_x, _x,_x,_x,_x, _x,_x,_x,_x, _x,_x,_x,_x, _x,_x,_x,_x, _x,_x,_x,_x, _x,_x,_x,_x, _x,_x,_x,_x, _x,_x,_x,_x, _x,_T,_T,_T, _x,_x,_x,_x, _x,_x,_x,_x, _x,_x,_x,_x, _x,_x,_x,_x, _x,_x,_x,_x, _x,_x,_x,_x, _x,_x,_x,_x, _x,_x,_x,_x, _x,_x,_x,_x, _x,_x,_x,_x, _x,_x,_x,_x, _x,_x,_x,_x, _x,_x,_x},
-		{_x,_x,_x,_x, _x,_x,_x,_x, _x,_x,_x,_x, _x,_x,_x,_x, _x,_x,_x,_x, _x,_x,_x,_x, _x,_x,_x,_x, _x,_x,_x,_x, _x,_x,_x,_x, _x,_x,_x,_x, _x,_x,_x,_T, _T,_T,_x,_x, _x,_x,_x,_x, _x,_x,_x,_x, _x,_x,_x,_x, _x,_x,_x,_x, _x,_x,_x,_x, _x,_x,_x,_x, _x,_x,_x,_x, _x,_x,_x,_x, _x,_x,_x,_x, _x,_x,_x,_x, _x,_x,_x,_x, _x,_T,_T,_T, _T,_x,_x,_x, _x,_x,_x,_x, _x,_x,_x,_x, _x,_x,_x,_x, _x,_x,_x,_x, _x,_x,_x,_x, _x,_x,_x,_x, _x,_x,_x,_x, _x,_x,_x,_x, _x,_x,_x,_x, _x,_x,_x,_x, _x,_x,_x,_x, _x,_x,_x,_x, _x,_x,_x},
-		{_x,_T,_T,_T, _T,_x,_x,_x, _x,_T,_x,_T, _x,_x,_T,_T, _T,_x,_T,_T, _T,_T,_x,_x, _T,_x,_x,_x, _x,_x,_x,_x, _x,_T,_T,_x, _x,_x,_x,_x, _x,_x,_x,_x, _x,_x,_x,_x, _x,_x,_T,_x, _T,_x,_T,_x, _x,_x,_x,_x, _x,_x,_x,_x, _T,_x,_x,_T, _x,_x,_x,_x, _x,_x,_x,_x, _x,_x,_x,_x, _x,_x,_x,_x, _T,_x,_x,_x, _x,_x,_x,_x, _x,_x,_x,_x, _x,_x,_x,_x, _T,_x,_x,_x, _T,_x,_T,_T, _x,_x,_T,_x, _x,_x,_x,_x, _x,_x,_x,_x, _x,_x,_x,_x, _T,_T,_T,_T, _T,_T,_T,_T, _T,_x,_x,_T, _x,_x,_x,_x, _T,_T,_T,_T, _T,_T,_T,_T, _x,_x,_x},
-		{_T,_x,_x,_x, _x,_x,_x,_x, _x,_x,_x,_x, _x,_x,_x,_x, _x,_x,_x,_x, _x,_x,_T,_x, _x,_x,_x,_x, _x,_x,_x,_x, _x,_x,_x,_x, _x,_x,_x,_T, _x,_T,_T,_T, _T,_T,_T,_x, _T,_T,_T,_T, _x,_x,_T,_x, _T,_x,_x,_x, _x,_x,_x,_x, _x,_x,_T,_T, _T,_T,_T,_T, _x,_T,_x,_x, _T,_x,_x,_x, _T,_T,_T,_T, _T,_T,_x,_T, _T,_x,_T,_x, _x,_T,_T,_T, _T,_x,_T,_x, _x,_x,_x,_x, _x,_x,_x,_x, _x,_x,_x,_x, _x,_x,_x,_x, _x,_x,_x,_x, _x,_x,_x,_x, _x,_x,_x,_x, _x,_x,_x,_x, _x,_x,_x,_x, _x,_x,_x,_x, _x,_x,_x,_x, _x,_x,_x,_x, _x,_x,_x},
-		{_x,_x,_x,_x, _x,_x,_x,_x, _x,_x,_x,_x, _x,_x,_x,_x, _x,_x,_x,_x, _x,_x,_x,_x, _x,_x,_x,_x, _x,_x,_x,_x, _x,_x,_x,_x, _x,_x,_x,_T, _x,_x,_x,_x, _x,_x,_x,_x, _T,_T,_x,_x, _x,_x,_x,_x, _x,_x,_x,_x, _x,_x,_x,_x, _x,_x,_x,_x, _x,_x,_x,_x, _x,_x,_x,_x, _x,_x,_x,_x, _x,_x,_x,_x, _x,_x,_x,_x, _x,_x,_x,_x, _x,_x,_x,_x, _x,_x,_T,_x, _x,_x,_x,_x, _x,_x,_x,_x, _x,_x,_x,_x, _x,_x,_x,_x, _x,_x,_x,_x, _x,_x,_x,_x, _x,_x,_x,_x, _x,_x,_x,_x, _x,_x,_x,_x, _x,_x,_x,_x, _x,_x,_x,_x, _x,_x,_x,_x, _x,_x,_x},
-		{_T,_x,_x,_x, _x,_x,_x,_x, _x,_x,_x,_x, _x,_x,_x,_x, _x,_x,_x,_x, _x,_x,_x,_x, _x,_x,_x,_x, _x,_x,_x,_x, _x,_x,_x,_x, _x,_x,_x,_x, _x,_x,_x,_T, _T,_T,_x,_x, _x,_x,_x,_x, _x,_x,_x,_x, _x,_x,_x,_x, _x,_x,_x,_x, _x,_x,_x,_x, _x,_x,_x,_x, _x,_x,_x,_x, _x,_x,_x,_x, _x,_x,_x,_x, _x,_x,_x,_x, _x,_x,_x,_x, _x,_T,_T,_T, _T,_x,_x,_x, _x,_x,_x,_x, _x,_x,_x,_x, _x,_x,_x,_x, _x,_x,_x,_x, _x,_x,_x,_x, _x,_x,_x,_x, _x,_x,_x,_x, _x,_x,_x,_x, _x,_x,_x,_x, _x,_x,_x,_x, _x,_x,_x,_x, _x,_x,_x,_x, _x,_x,_x},
-		{_x,_x,_x,_x, _x,_x,_x,_x, _x,_x,_x,_x, _x,_x,_x,_x, _x,_x,_x,_x, _x,_x,_x,_x, _x,_x,_x,_x, _x,_x,_x,_x, _x,_x,_x,_x, _x,_x,_x,_T, _x,_x,_x,_x, _x,_x,_x,_T, _x,_T,_x,_x, _x,_x,_x,_x, _x,_x,_x,_x, _x,_x,_x,_x, _x,_x,_x,_x, _x,_x,_x,_x, _x,_x,_x,_x, _x,_x,_x,_x, _x,_x,_x,_x, _x,_x,_x,_x, _x,_x,_x,_x, _x,_x,_x,_x, _x,_T,_T,_x, _x,_x,_x,_x, _x,_x,_x,_x, _x,_x,_x,_x, _x,_x,_x,_x, _x,_x,_x,_x, _x,_x,_x,_x, _x,_x,_x,_x, _x,_x,_x,_x, _x,_x,_x,_x, _x,_x,_x,_x, _x,_x,_x,_x, _x,_x,_x,_x, _x,_x,_x},
-		{_x,_T,_T,_x, _x,_T,_T,_T, _T,_T,_T,_T, _T,_T,_T,_T, _T,_T,_T,_T, _x,_x,_x,_x, _x,_x,_x,_x, _x,_x,_x,_x, _x,_x,_x,_x, _x,_x,_x,_x, _x,_x,_x,_x, _x,_x,_x,_x, _x,_x,_x,_x, _x,_x,_T,_x, _x,_x,_x,_x, _x,_x,_x,_x, _x,_x,_x,_T, _x,_x,_x,_x, _x,_x,_x,_x, _x,_x,_x,_x, _x,_x,_x,_x, _x,_x,_x,_x, _x,_x,_x,_x, _x,_x,_x,_x, _x,_x,_x,_x, _x,_x,_x,_x, _x,_x,_x,_x, _x,_x,_x,_x, _x,_x,_x,_x, _x,_x,_x,_x, _x,_x,_x,_x, _x,_x,_x,_x, _x,_x,_x,_x, _x,_x,_x,_x, _x,_x,_x,_x, _x,_x,_x,_x, _x,_x,_x,_x, _x,_x,_x},
-		{_T,_x,_x,_x, _x,_x,_x,_x, _x,_x,_x,_x, _x,_x,_x,_x, _x,_x,_x,_x, _x,_x,_x,_x, _x,_x,_x,_x, _x,_x,_x,_x, _x,_x,_x,_x, _x,_x,_x,_T, _x,_x,_x,_x, _x,_x,_x,_T, _T,_T,_x,_x, _x,_x,_x,_x, _x,_x,_x,_x, _x,_x,_x,_x, _x,_x,_x,_x, _x,_x,_x,_x, _x,_x,_x,_x, _x,_x,_x,_x, _x,_x,_x,_x, _x,_x,_x,_x, _x,_x,_x,_x, _x,_x,_x,_x, _x,_T,_T,_T, _x,_x,_x,_x, _x,_x,_x,_x, _x,_x,_x,_x, _x,_x,_x,_x, _x,_x,_x,_x, _x,_x,_x,_x, _x,_x,_x,_x, _x,_x,_x,_x, _x,_x,_x,_x, _x,_x,_x,_x, _x,_x,_x,_x, _x,_x,_x,_x, _x,_x,_x},
-		{_x,_x,_x,_x, _x,_x,_x,_x, _x,_x,_x,_x, _x,_x,_x,_x, _x,_x,_x,_x, _x,_x,_x,_x, _x,_x,_x,_x, _x,_x,_x,_x, _x,_x,_x,_x, _x,_x,_x,_x, _x,_x,_x,_x, _x,_x,_x,_x, _x,_T,_x,_x, _x,_x,_x,_x, _x,_x,_x,_x, _x,_x,_x,_x, _x,_x,_x,_x, _x,_x,_x,_x, _x,_x,_x,_x, _x,_x,_x,_x, _x,_x,_x,_x, _x,_x,_x,_x, _x,_x,_x,_x, _x,_x,_x,_x, _x,_T,_T,_T, _x,_x,_x,_x, _x,_x,_x,_x, _x,_x,_x,_x, _x,_x,_x,_x, _x,_x,_x,_x, _x,_x,_x,_x, _x,_x,_x,_x, _x,_x,_x,_x, _x,_x,_x,_x, _x,_x,_x,_x, _x,_x,_x,_x, _x,_x,_x,_x, _x,_x,_x},
-		{_x,_T,_T,_T, _T,_x,_x,_x, _x,_T,_x,_T, _x,_x,_x,_x, _x,_x,_x,_x, _T,_T,_x,_x, _T,_x,_x,_x, _x,_x,_x,_x, _x,_T,_T,_x, _x,_x,_x,_x, _x,_x,_x,_x, _x,_x,_x,_x, _x,_x,_T,_x, _x,_x,_T,_x, _x,_x,_x,_x, _x,_x,_x,_T, _T,_x,_x,_T, _x,_x,_x,_x, _x,_x,_x,_x, _x,_x,_x,_x, _x,_x,_x,_x, _T,_x,_x,_x, _x,_x,_x,_x, _x,_x,_x,_x, _x,_x,_x,_T, _T,_T,_x,_T, _T,_T,_T,_T, _x,_T,_T,_T, _T,_x,_x,_x, _x,_x,_x,_x, _x,_x,_x,_x, _x,_x,_x,_x, _x,_x,_x,_x, _x,_x,_x,_x, _x,_x,_x,_x, _T,_T,_T,_T, _T,_T,_T,_T, _x,_x,_x},
-		{_T,_x,_x,_x, _x,_x,_x,_x, _x,_x,_x,_x, _x,_x,_x,_x, _x,_x,_x,_x, _x,_x,_x,_x, _x,_x,_x,_x, _x,_x,_x,_x, _x,_x,_x,_x, _x,_x,_x,_T, _x,_x,_x,_x, _x,_x,_x,_T, _x,_T,_x,_x, _x,_x,_x,_x, _x,_x,_x,_x, _x,_x,_x,_x, _x,_x,_x,_x, _x,_x,_x,_x, _x,_x,_x,_x, _x,_x,_x,_x, _x,_x,_x,_x, _x,_x,_x,_x, _x,_x,_x,_x, _x,_x,_x,_x, _x,_T,_T,_x, _x,_x,_x,_x, _x,_x,_x,_x, _x,_x,_x,_x, _x,_x,_x,_x, _x,_x,_x,_x, _x,_x,_x,_x, _x,_x,_x,_x, _x,_x,_x,_x, _x,_x,_x,_x, _x,_x,_x,_x, _x,_x,_x,_x, _x,_x,_x,_x, _x,_x,_x},
-		{_T,_x,_x,_x, _x,_x,_x,_x, _x,_x,_x,_x, _x,_x,_x,_x, _x,_x,_x,_x, _x,_x,_x,_x, _x,_x,_x,_x, _x,_x,_x,_x, _x,_x,_x,_x, _x,_x,_x,_T, _x,_x,_x,_x, _x,_x,_x,_x, _T,_T,_x,_x, _x,_x,_x,_x, _x,_x,_x,_x, _x,_x,_x,_x, _x,_x,_x,_x, _x,_x,_x,_x, _x,_x,_x,_x, _x,_x,_x,_x, _x,_x,_x,_x, _x,_x,_x,_x, _x,_x,_x,_x, _x,_x,_x,_x, _x,_x,_T,_x, _x,_x,_x,_x, _x,_x,_x,_x, _x,_x,_x,_x, _x,_x,_x,_x, _x,_x,_x,_x, _x,_x,_x,_x, _x,_x,_x,_x, _x,_x,_x,_x, _x,_x,_x,_x, _x,_x,_x,_x, _x,_x,_x,_x, _x,_x,_x,_x, _x,_x,_x},
-		{_x,_T,_T,_T, _T,_x,_x,_x, _x,_T,_x,_T, _x,_x,_T,_T, _T,_x,_T,_T, _T,_T,_x,_x, _T,_x,_x,_x, _x,_T,_x,_x, _x,_T,_T,_x, _x,_x,_x,_x, _x,_x,_x,_x, _x,_x,_x,_x, _x,_x,_T,_x, _T,_x,_T,_x, _x,_x,_x,_x, _x,_x,_x,_x, _T,_x,_x,_T, _x,_x,_x,_x, _x,_x,_x,_x, _x,_x,_x,_x, _x,_x,_x,_x, _T,_x,_x,_x, _x,_x,_x,_x, _x,_x,_x,_x, _x,_x,_x,_x, _T,_x,_x,_x, _T,_x,_T,_T, _x,_x,_T,_x, _x,_x,_x,_x, _x,_x,_x,_x, _x,_x,_x,_x, _T,_T,_T,_T, _T,_T,_T,_T, _T,_x,_x,_T, _x,_x,_x,_x, _T,_T,_T,_T, _T,_T,_T,_T, _x,_x,_x},
-		{_T,_T,_T,_T, _T,_x,_x,_x, _x,_T,_x,_T, _x,_x,_x,_x, _x,_x,_x,_x, _T,_T,_x,_x, _T,_x,_x,_x, _x,_x,_x,_x, _x,_T,_T,_x, _x,_x,_x,_x, _x,_x,_x,_x, _x,_x,_x,_x, _x,_x,_T,_x, _x,_x,_T,_x, _x,_x,_x,_x, _x,_x,_x,_T, _T,_x,_x,_T, _x,_x,_x,_x, _x,_x,_x,_x, _x,_x,_x,_x, _x,_x,_x,_x, _T,_x,_x,_x, _x,_x,_x,_x, _x,_x,_x,_x, _x,_x,_x,_T, _T,_T,_x,_T, _T,_T,_T,_T, _x,_T,_T,_T, _T,_x,_x,_x, _x,_x,_x,_x, _x,_x,_x,_x, _x,_x,_x,_x, _x,_x,_x,_x, _x,_x,_x,_x, _x,_x,_x,_x, _T,_T,_T,_T, _T,_T,_T,_T, _x,_x,_x},
-		{_x,_T,_T,_T, _T,_x,_x,_x, _x,_T,_x,_T, _x,_x,_T,_T, _T,_x,_T,_T, _T,_T,_x,_x, _T,_x,_x,_x, _x,_x,_x,_x, _x,_T,_T,_x, _x,_x,_x,_x, _x,_x,_x,_x, _x,_x,_x,_x, _x,_x,_T,_x, _T,_x,_T,_x, _x,_x,_x,_x, _x,_T,_x,_T, _T,_x,_x,_T, _x,_x,_x,_x, _x,_x,_x,_x, _x,_x,_x,_x, _x,_x,_x,_x, _T,_x,_x,_x, _x,_x,_x,_x, _x,_x,_x,_x, _x,_x,_x,_x, _T,_x,_x,_x, _T,_x,_T,_T, _x,_x,_T,_x, _x,_x,_x,_x, _x,_x,_x,_x, _x,_x,_x,_x, _T,_T,_T,_T, _T,_T,_T,_T, _T,_x,_x,_T, _x,_x,_x,_x, _T,_T,_T,_T, _T,_T,_T,_T, _x,_x,_x},
-		{_x,_T,_T,_T, _T,_x,_x,_x, _x,_T,_x,_T, _x,_x,_T,_T, _T,_x,_T,_T, _T,_T,_x,_x, _T,_x,_x,_x, _x,_x,_x,_x, _x,_T,_T,_x, _x,_x,_x,_x, _x,_x,_x,_x, _x,_x,_x,_x, _x,_x,_T,_x, _T,_x,_T,_x, _x,_x,_x,_x, _x,_T,_x,_x, _T,_x,_x,_T, _x,_x,_x,_x, _x,_x,_x,_x, _x,_x,_x,_x, _x,_x,_x,_x, _T,_x,_x,_x, _x,_x,_x,_x, _x,_x,_x,_x, _x,_x,_x,_x, _T,_x,_x,_x, _T,_x,_T,_T, _x,_x,_T,_x, _x,_x,_x,_x, _x,_x,_x,_x, _x,_x,_x,_x, _T,_T,_T,_T, _T,_T,_T,_T, _T,_x,_x,_T, _x,_x,_x,_x, _T,_T,_T,_T, _T,_T,_T,_T, _x,_x,_x},
-		{_x,_x,_x,_x, _x,_x,_x,_x, _x,_x,_x,_x, _x,_x,_x,_x, _x,_x,_x,_x, _x,_x,_x,_x, _x,_x,_x,_x, _x,_x,_x,_x, _x,_x,_x,_x, _x,_x,_x,_T, _T,_x,_x,_x, _x,_x,_x,_T, _x,_x,_x,_x, _x,_x,_x,_x, _x,_x,_x,_x, _x,_x,_x,_x, _x,_x,_x,_x, _x,_x,_x,_x, _x,_x,_x,_x, _x,_x,_x,_x, _x,_x,_x,_x, _x,_x,_x,_x, _x,_x,_x,_x, _x,_x,_x,_x, _x,_T,_x,_x, _x,_x,_x,_x, _x,_x,_x,_x, _x,_x,_x,_x, _x,_x,_x,_x, _x,_x,_x,_x, _x,_x,_x,_x, _x,_x,_x,_x, _x,_x,_x,_x, _x,_x,_x,_x, _x,_x,_x,_x, _x,_x,_x,_x, _x,_x,_x,_x, _x,_x,_x},
-		{_x,_T,_T,_T, _T,_x,_x,_x, _x,_T,_x,_T, _x,_x,_x,_x, _x,_x,_x,_x, _T,_T,_x,_x, _T,_x,_x,_x, _x,_x,_x,_x, _x,_T,_T,_T, _x,_x,_x,_x, _x,_x,_x,_x, _x,_x,_x,_x, _x,_x,_T,_T, _x,_x,_T,_x, _x,_x,_x,_x, _x,_x,_x,_T, _T,_x,_x,_T, _x,_x,_x,_x, _x,_x,_x,_x, _x,_x,_x,_x, _x,_x,_x,_x, _T,_x,_x,_x, _x,_x,_x,_x, _x,_x,_x,_x, _x,_x,_x,_T, _T,_T,_x,_T, _T,_T,_T,_T, _x,_T,_T,_T, _T,_x,_x,_x, _x,_x,_x,_x, _x,_x,_x,_x, _x,_x,_x,_x, _x,_x,_x,_x, _x,_x,_x,_x, _x,_x,_x,_x, _T,_T,_T,_T, _T,_T,_T,_T, _x,_x,_x},
-		{_x,_T,_T,_T, _T,_x,_x,_x, _x,_T,_x,_T, _x,_x,_x,_x, _x,_x,_x,_x, _T,_T,_x,_x, _T,_x,_x,_x, _x,_x,_x,_x, _x,_T,_T,_T, _x,_x,_x,_x, _x,_x,_x,_x, _x,_x,_x,_x, _x,_x,_T,_T, _x,_x,_T,_x, _x,_x,_x,_x, _x,_x,_x,_T, _T,_x,_x,_T, _x,_x,_x,_x, _x,_x,_x,_x, _x,_x,_x,_x, _x,_x,_x,_x, _T,_x,_x,_x, _x,_x,_x,_x, _x,_x,_x,_x, _x,_T,_T,_T, _T,_T,_x,_T, _T,_T,_T,_T, _x,_T,_T,_T, _T,_x,_x,_x, _x,_x,_x,_x, _x,_x,_x,_x, _x,_x,_x,_x, _x,_x,_x,_x, _x,_x,_x,_x, _x,_x,_x,_x, _T,_T,_T,_T, _T,_T,_T,_T, _x,_x,_x},
-		{_x,_x,_x,_x, _x,_x,_x,_x, _x,_x,_x,_x, _x,_x,_x,_x, _x,_x,_x,_x, _x,_x,_x,_x, _x,_x,_x,_x, _x,_x,_x,_x, _x,_x,_x,_x, _x,_x,_x,_x, _x,_x,_x,_x, _x,_x,_x,_x, _x,_x,_x,_x, _x,_x,_x,_x, _T,_T,_T,_T, _T,_x,_x,_x, _x,_x,_x,_x, _x,_x,_x,_x, _x,_x,_x,_x, _x,_x,_x,_x, _x,_x,_x,_x, _x,_x,_x,_x, _x,_x,_x,_x, _x,_x,_x,_x, _x,_x,_x,_x, _x,_x,_x,_x, _x,_x,_x,_x, _x,_x,_x,_x, _x,_x,_T,_T, _T,_T,_T,_T, _T,_T,_T,_T, _x,_x,_x,_x, _x,_x,_x,_x, _x,_x,_x,_x, _x,_x,_x,_x, _x,_x,_x,_x, _x,_x,_x,_x, _x,_x,_x},
-		{_x,_T,_T,_T, _T,_x,_x,_x, _x,_T,_x,_T, _x,_x,_T,_T, _T,_x,_T,_T, _T,_T,_x,_x, _T,_x,_x,_x, _x,_x,_x,_x, _x,_T,_T,_x, _x,_x,_x,_x, _x,_x,_x,_x, _x,_x,_x,_x, _x,_x,_T,_x, _T,_x,_T,_x, _x,_x,_x,_x, _x,_T,_x,_x, _T,_x,_x,_T, _x,_x,_x,_x, _x,_x,_x,_x, _x,_x,_x,_x, _x,_x,_x,_x, _T,_x,_x,_x, _x,_T,_x,_x, _x,_x,_x,_x, _x,_x,_x,_x, _T,_x,_x,_x, _T,_x,_T,_T, _x,_x,_T,_x, _x,_x,_x,_x, _x,_x,_x,_x, _x,_x,_x,_x, _T,_T,_T,_T, _T,_T,_T,_T, _T,_x,_x,_T, _x,_x,_x,_x, _T,_T,_T,_T, _T,_T,_T,_T, _x,_x,_x},
-		{_x,_x,_T,_T, _T,_x,_x,_x, _x,_T,_x,_T, _x,_x,_x,_x, _x,_x,_x,_x, _T,_T,_x,_x, _T,_x,_x,_x, _x,_x,_x,_x, _x,_x,_x,_x, _x,_x,_x,_x, _x,_x,_x,_x, _x,_x,_x,_x, _x,_x,_x,_x, _x,_x,_T,_x, _x,_x,_x,_x, _x,_x,_x,_x, _x,_x,_x,_x, _x,_x,_x,_x, _x,_x,_x,_x, _x,_x,_x,_x, _x,_x,_x,_x, _x,_x,_x,_x, _x,_x,_x,_x, _x,_x,_x,_x, _x,_x,_x,_x, _x,_x,_x,_x, _x,_x,_x,_x, _x,_x,_x,_x, _x,_x,_x,_x, _x,_x,_x,_x, _x,_x,_x,_x, _x,_x,_x,_x, _x,_x,_x,_x, _x,_x,_x,_x, _x,_x,_x,_x, _T,_T,_T,_T, _T,_T,_T,_T, _x,_x,_x},
-		{_T,_T,_T,_T, _T,_x,_x,_x, _x,_T,_x,_T, _x,_x,_x,_x, _x,_x,_x,_x, _T,_T,_x,_x, _T,_x,_x,_x, _x,_x,_x,_x, _x,_T,_T,_T, _x,_x,_x,_x, _x,_x,_x,_x, _x,_x,_x,_x, _x,_x,_T,_T, _x,_x,_T,_x, _x,_x,_x,_x, _x,_x,_x,_T, _T,_x,_x,_T, _x,_x,_x,_x, _x,_x,_x,_x, _x,_x,_x,_x, _x,_x,_x,_x, _T,_x,_x,_x, _x,_x,_x,_x, _x,_x,_x,_x, _x,_x,_x,_T, _T,_T,_x,_T, _T,_T,_T,_T, _x,_T,_T,_T, _T,_x,_x,_x, _x,_x,_x,_x, _x,_x,_x,_x, _x,_x,_x,_x, _x,_x,_x,_x, _x,_x,_x,_x, _x,_x,_x,_x, _T,_T,_T,_T, _T,_T,_T,_T, _x,_x,_x},
-		{_x,_T,_T,_T, _T,_x,_x,_x, _x,_T,_x,_T, _x,_x,_T,_T, _T,_x,_T,_T, _T,_T,_x,_x, _T,_x,_x,_x, _x,_x,_x,_x, _x,_T,_T,_x, _x,_x,_x,_x, _x,_x,_x,_x, _x,_x,_x,_x, _x,_x,_T,_x, _T,_x,_T,_x, _x,_x,_x,_x, _x,_x,_x,_x, _T,_x,_x,_T, _x,_x,_x,_x, _x,_x,_x,_x, _x,_x,_x,_x, _x,_x,_x,_x, _T,_x,_x,_x, _x,_x,_x,_x, _x,_x,_x,_x, _x,_x,_x,_x, _T,_x,_x,_x, _T,_x,_T,_T, _x,_x,_T,_x, _x,_x,_x,_x, _x,_x,_x,_x, _x,_x,_x,_x, _x,_x,_x,_x, _T,_T,_T,_T, _T,_x,_x,_T, _x,_x,_x,_x, _T,_T,_T,_T, _T,_T,_T,_T, _x,_x,_x},
-		{_x,_x,_x,_x, _x,_x,_x,_x, _x,_x,_x,_x, _x,_x,_T,_T, _x,_x,_T,_T, _x,_x,_x,_x, _x,_x,_x,_x, _x,_x,_x,_x, _x,_T,_T,_x, _x,_x,_x,_x, _x,_x,_x,_x, _x,_x,_x,_x, _x,_x,_x,_x, _x,_x,_x,_x, _x,_x,_x,_x, _x,_x,_x,_x, _T,_x,_x,_T, _x,_x,_x,_x, _x,_x,_x,_x, _x,_x,_x,_x, _x,_x,_x,_x, _T,_x,_x,_x, _x,_x,_x,_x, _x,_x,_x,_x, _x,_x,_x,_x, _T,_x,_x,_x, _T,_x,_T,_T, _x,_x,_T,_x, _x,_x,_x,_x, _x,_x,_x,_x, _x,_x,_x,_x, _x,_x,_x,_x, _x,_x,_T,_T, _T,_x,_x,_x, _x,_x,_x,_x, _x,_x,_x,_x, _x,_x,_x,_x, _x,_x,_x},
-		{_T,_T,_T,_T, _T,_x,_x,_x, _x,_T,_x,_T, _x,_x,_x,_x, _x,_x,_x,_x, _T,_T,_T,_T, _T,_T,_T,_T, _T,_T,_T,_T, _T,_T,_T,_T, _T,_T,_T,_T, _T,_T,_T,_T, _T,_T,_T,_T, _T,_T,_T,_T, _T,_T,_T,_T, _T,_T,_T,_T, _T,_T,_T,_T, _T,_x,_T,_T, _T,_T,_T,_T, _x,_T,_x,_x, _T,_x,_x,_x, _T,_T,_T,_T, _T,_T,_T,_T, _T,_x,_T,_x, _x,_T,_T,_T, _T,_T,_T,_T, _T,_T,_x,_T, _T,_T,_T,_T, _T,_T,_T,_T, _T,_x,_T,_T, _T,_T,_T,_T, _T,_T,_T,_T, _T,_T,_T,_T, _T,_x,_x,_x, _x,_T,_T,_T, _T,_T,_T,_T, _T,_T,_T,_T, _T,_T,_T,_T, _T,_x,_x},
-		{_T,_T,_T,_T, _T,_x,_x,_x, _x,_T,_x,_T, _x,_x,_x,_x, _x,_x,_x,_x, _T,_T,_T,_T, _T,_T,_x,_T, _x,_T,_T,_T, _T,_T,_T,_T, _T,_T,_T,_T, _T,_T,_T,_T, _T,_T,_T,_T, _T,_T,_T,_T, _x,_T,_T,_T, _T,_T,_T,_T, _T,_T,_T,_T, _T,_x,_T,_T, _T,_T,_T,_T, _x,_T,_x,_x, _T,_x,_x,_x, _T,_T,_T,_T, _T,_T,_T,_T, _T,_x,_T,_x, _x,_T,_T,_T, _T,_T,_T,_T, _T,_T,_x,_T, _T,_T,_T,_T, _T,_T,_T,_T, _T,_x,_T,_T, _T,_T,_T,_T, _T,_T,_T,_T, _T,_T,_T,_T, _T,_x,_x,_x, _x,_T,_T,_T, _T,_T,_T,_T, _T,_T,_T,_T, _T,_T,_T,_T, _T,_x,_x}
+		{_T,_T,_T,_T, _T,_x,_x,_x, _x,_T,_x,_T, _x,_x,_x,_x, _x,_x,_x,_x, _T,_T,_x,_x, _T,_x,_x,_x, _x,_x,_T,_x, _x,_T,_T,_T, _x,_x,_x,_T, _T,_x,_x,_T, _T,_T,_x,_T, _T,_T,_T,_T, _x,_x,_T,_x, _x,_x,_x,_x, _x,_x,_x,_T, _T,_x,_x,_T, _x,_x,_x,_x, _x,_x,_x,_x, _x,_x,_x,_x, _T,_T,_T,_T, _T,_T,_x,_x, _x,_x,_x,_T, _x,_x,_T,_T, _T,_T,_T,_T, _T,_T,_T,_x, _T,_T,_T,_T, _T,_x,_T,_T, _T,_T,_x,_x, _x,_x,_x,_x, _x,_x,_x,_x, _x,_x,_x,_x, _x,_x,_x,_x, _x,_x,_x,_x, _x,_x,_x,_x, _x,_T,_T,_T, _T,_T,_T,_T, _T,_x,_x,_x},
+		{_x,_x,_x,_x, _x,_x,_x,_x, _x,_x,_x,_x, _x,_x,_x,_x, _x,_x,_x,_x, _x,_x,_x,_x, _x,_x,_x,_x, _x,_x,_x,_x, _x,_x,_x,_x, _x,_x,_x,_x, _x,_T,_T,_T, _T,_T,_T,_x, _x,_x,_x,_x, _x,_x,_x,_x, _x,_x,_x,_x, _x,_x,_x,_x, _x,_x,_T,_T, _T,_T,_T,_T, _x,_T,_x,_x, _T,_x,_x,_x, _T,_T,_T,_T, _T,_T,_x,_T, _x,_T,_x,_T, _x,_x,_T,_T, _T,_T,_x,_x, _x,_x,_x,_x, _x,_x,_x,_x, _x,_x,_x,_x, _x,_x,_x,_x, _x,_x,_x,_x, _x,_x,_x,_x, _x,_x,_x,_x, _x,_x,_x,_x, _x,_x,_x,_x, _x,_x,_x,_x, _x,_x,_x,_x, _x,_x,_x,_x, _x,_x,_x,_x},
+		{_x,_x,_x,_x, _x,_x,_x,_x, _x,_x,_x,_x, _x,_x,_x,_x, _x,_x,_x,_x, _x,_x,_x,_x, _x,_x,_x,_x, _x,_x,_x,_x, _x,_x,_x,_x, _x,_x,_x,_x, _x,_x,_x,_x, _x,_x,_x,_x, _x,_x,_x,_x, _x,_x,_x,_x, _x,_x,_x,_x, _x,_x,_x,_x, _x,_x,_T,_T, _T,_T,_T,_x, _x,_x,_x,_x, _x,_x,_x,_x, _x,_x,_x,_x, _x,_x,_x,_x, _x,_x,_x,_x, _x,_x,_x,_x, _x,_x,_x,_x, _x,_x,_x,_x, _x,_x,_x,_x, _x,_x,_x,_x, _x,_x,_x,_x, _x,_x,_x,_x, _x,_x,_x,_x, _x,_x,_x,_x, _x,_x,_x,_x, _x,_x,_x,_x, _x,_x,_x,_x, _x,_x,_x,_x, _x,_x,_x,_x, _x,_x,_x,_x},
+		{_T,_x,_x,_x, _x,_x,_x,_x, _x,_x,_x,_x, _x,_x,_x,_x, _x,_x,_x,_x, _x,_x,_x,_x, _x,_x,_x,_x, _T,_T,_T,_x, _x,_x,_x,_x, _x,_x,_x,_x, _x,_T,_T,_T, _T,_T,_T,_x, _x,_x,_x,_T, _x,_x,_x,_x, _x,_x,_x,_x, _x,_x,_x,_x, _x,_x,_T,_T, _T,_T,_T,_T, _x,_T,_x,_x, _T,_x,_x,_x, _T,_T,_T,_T, _T,_T,_x,_T, _x,_T,_x,_T, _x,_x,_T,_T, _T,_T,_x,_x, _x,_x,_x,_x, _x,_x,_x,_x, _x,_x,_x,_x, _x,_x,_x,_x, _x,_x,_x,_x, _x,_x,_x,_x, _x,_x,_x,_x, _x,_x,_x,_x, _x,_x,_x,_x, _x,_x,_x,_x, _x,_x,_x,_x, _x,_x,_x,_x, _x,_x,_x,_x},
+		{_x,_T,_T,_x, _T,_x,_x,_x, _x,_x,_x,_x, _x,_x,_x,_x, _x,_x,_x,_x, _x,_x,_x,_x, _x,_x,_x,_x, _x,_x,_x,_x, _x,_x,_x,_x, _x,_x,_x,_x, _x,_x,_x,_x, _x,_x,_x,_x, _T,_T,_x,_x, _x,_x,_x,_x, _x,_x,_x,_x, _x,_x,_x,_x, _x,_x,_x,_x, _x,_x,_x,_x, _x,_x,_x,_x, _x,_x,_x,_x, _x,_x,_x,_x, _x,_x,_x,_x, _x,_x,_x,_x, _x,_x,_x,_x, _x,_x,_x,_x, _x,_x,_x,_x, _x,_x,_x,_x, _x,_x,_x,_x, _x,_x,_x,_x, _x,_x,_x,_x, _x,_x,_x,_x, _x,_x,_x,_x, _x,_x,_x,_x, _x,_x,_x,_x, _x,_x,_x,_x, _x,_x,_x,_x, _x,_x,_x,_x, _x,_x,_x,_x},
+		{_x,_x,_x,_x, _x,_x,_x,_x, _x,_x,_x,_x, _x,_x,_x,_x, _x,_x,_x,_x, _x,_x,_x,_x, _x,_x,_x,_x, _x,_x,_x,_x, _x,_x,_x,_x, _x,_x,_x,_x, _x,_T,_T,_T, _T,_T,_T,_x, _x,_x,_x,_x, _x,_x,_x,_x, _x,_x,_x,_x, _x,_x,_x,_x, _x,_x,_T,_T, _T,_T,_T,_x, _x,_x,_x,_x, _x,_x,_x,_x, _x,_x,_x,_x, _T,_T,_x,_x, _x,_x,_x,_x, _x,_x,_T,_T, _T,_T,_x,_x, _x,_x,_x,_x, _x,_x,_x,_x, _x,_x,_x,_x, _x,_x,_x,_x, _x,_x,_x,_x, _x,_x,_x,_x, _x,_x,_x,_x, _x,_x,_x,_x, _x,_x,_x,_x, _x,_x,_x,_x, _x,_x,_x,_x, _x,_x,_x,_x, _x,_x,_x,_x},
+		{_x,_T,_x,_x, _x,_T,_T,_T, _T,_T,_T,_T, _T,_T,_T,_T, _T,_T,_T,_T, _x,_x,_x,_x, _x,_x,_x,_x, _x,_x,_x,_x, _x,_x,_x,_x, _x,_x,_x,_x, _x,_x,_x,_x, _x,_x,_x,_x, _x,_x,_x,_x, _x,_x,_T,_x, _x,_x,_x,_x, _x,_x,_x,_x, _x,_x,_x,_x, _x,_x,_x,_x, _x,_x,_x,_x, _x,_x,_x,_x, _x,_x,_x,_x, _x,_x,_x,_x, _x,_x,_x,_x, _x,_x,_x,_x, _x,_x,_x,_x, _x,_x,_x,_x, _x,_x,_x,_x, _x,_x,_x,_x, _x,_x,_x,_x, _x,_x,_x,_x, _x,_x,_x,_x, _x,_x,_x,_x, _x,_x,_x,_x, _x,_x,_x,_x, _x,_x,_x,_x, _x,_x,_x,_x, _x,_x,_x,_x, _x,_x,_x,_x},
+		{_x,_x,_x,_x, _x,_x,_x,_x, _x,_x,_x,_x, _x,_x,_x,_x, _x,_x,_x,_x, _x,_x,_x,_x, _x,_x,_x,_x, _x,_x,_x,_x, _x,_x,_x,_x, _x,_x,_x,_T, _x,_x,_x,_x, _x,_x,_x,_T, _T,_T,_x,_x, _x,_x,_x,_x, _x,_x,_x,_x, _x,_x,_x,_x, _x,_x,_x,_x, _x,_x,_x,_x, _x,_x,_x,_x, _x,_x,_x,_x, _x,_x,_x,_x, _x,_x,_x,_x, _x,_x,_x,_x, _x,_x,_x,_x, _x,_x,_T,_T, _T,_x,_x,_x, _x,_x,_x,_x, _x,_x,_x,_x, _x,_x,_x,_x, _x,_x,_x,_x, _x,_x,_x,_x, _x,_x,_x,_x, _x,_x,_x,_x, _x,_x,_x,_x, _x,_x,_x,_x, _x,_x,_x,_x, _x,_x,_x,_x, _x,_x,_x,_x},
+		{_x,_x,_x,_x, _x,_x,_x,_x, _x,_x,_x,_x, _x,_x,_x,_x, _x,_x,_x,_x, _x,_x,_x,_x, _x,_x,_x,_x, _x,_x,_x,_x, _x,_x,_x,_x, _x,_x,_x,_x, _x,_x,_x,_T, _T,_T,_x,_x, _x,_x,_x,_x, _x,_x,_x,_x, _x,_x,_x,_x, _x,_x,_x,_x, _x,_x,_x,_x, _x,_x,_x,_x, _x,_x,_x,_x, _x,_x,_x,_x, _x,_x,_x,_x, _x,_x,_x,_x, _x,_x,_x,_x, _x,_x,_T,_T, _T,_T,_x,_x, _x,_x,_x,_x, _x,_x,_x,_x, _x,_x,_x,_x, _x,_x,_x,_x, _x,_x,_x,_x, _x,_x,_x,_x, _x,_x,_x,_x, _x,_x,_x,_x, _x,_x,_x,_x, _x,_x,_x,_x, _x,_x,_x,_x, _x,_x,_x,_x, _x,_x,_x,_x},
+		{_x,_T,_T,_T, _T,_x,_x,_x, _x,_T,_x,_T, _x,_x,_T,_T, _T,_x,_T,_T, _T,_T,_x,_x, _T,_x,_x,_x, _x,_x,_x,_x, _x,_T,_T,_x, _x,_x,_x,_x, _x,_x,_x,_x, _x,_x,_x,_x, _x,_x,_T,_x, _T,_x,_T,_x, _x,_x,_x,_x, _x,_x,_x,_x, _T,_x,_x,_T, _x,_x,_x,_x, _x,_x,_x,_x, _x,_x,_x,_x, _x,_x,_x,_x, _T,_x,_x,_x, _x,_x,_x,_x, _x,_x,_x,_x, _x,_x,_x,_x, _x,_T,_x,_x, _x,_T,_x,_T, _T,_x,_x,_T, _x,_x,_x,_x, _x,_x,_x,_x, _x,_x,_x,_x, _x,_T,_T,_T, _T,_T,_T,_T, _T,_T,_x,_x, _T,_x,_x,_x, _x,_T,_T,_T, _T,_T,_T,_T, _T,_x,_x,_x},
+		{_T,_x,_x,_x, _x,_x,_x,_x, _x,_x,_x,_x, _x,_x,_x,_x, _x,_x,_x,_x, _x,_x,_T,_x, _x,_x,_x,_x, _x,_x,_x,_x, _x,_x,_x,_x, _x,_x,_x,_T, _x,_T,_T,_T, _T,_T,_T,_x, _T,_T,_T,_T, _x,_x,_T,_x, _T,_x,_x,_x, _x,_x,_x,_x, _x,_x,_T,_T, _T,_T,_T,_T, _x,_T,_x,_x, _T,_x,_x,_x, _T,_T,_T,_T, _T,_T,_x,_T, _x,_T,_x,_T, _x,_x,_T,_T, _T,_T,_x,_T, _x,_x,_x,_x, _x,_x,_x,_x, _x,_x,_x,_x, _x,_x,_x,_x, _x,_x,_x,_x, _x,_x,_x,_x, _x,_x,_x,_x, _x,_x,_x,_x, _x,_x,_x,_x, _x,_x,_x,_x, _x,_x,_x,_x, _x,_x,_x,_x, _x,_x,_x,_x},
+		{_x,_x,_x,_x, _x,_x,_x,_x, _x,_x,_x,_x, _x,_x,_x,_x, _x,_x,_x,_x, _x,_x,_x,_x, _x,_x,_x,_x, _x,_x,_x,_x, _x,_x,_x,_x, _x,_x,_x,_T, _x,_x,_x,_x, _x,_x,_x,_x, _T,_T,_x,_x, _x,_x,_x,_x, _x,_x,_x,_x, _x,_x,_x,_x, _x,_x,_x,_x, _x,_x,_x,_x, _x,_x,_x,_x, _x,_x,_x,_x, _x,_x,_x,_x, _x,_x,_x,_x, _x,_x,_x,_x, _x,_x,_x,_x, _x,_x,_x,_T, _x,_x,_x,_x, _x,_x,_x,_x, _x,_x,_x,_x, _x,_x,_x,_x, _x,_x,_x,_x, _x,_x,_x,_x, _x,_x,_x,_x, _x,_x,_x,_x, _x,_x,_x,_x, _x,_x,_x,_x, _x,_x,_x,_x, _x,_x,_x,_x, _x,_x,_x,_x},
+		{_T,_x,_x,_x, _x,_x,_x,_x, _x,_x,_x,_x, _x,_x,_x,_x, _x,_x,_x,_x, _x,_x,_x,_x, _x,_x,_x,_x, _x,_x,_x,_x, _x,_x,_x,_x, _x,_x,_x,_x, _x,_x,_x,_T, _T,_T,_x,_x, _x,_x,_x,_x, _x,_x,_x,_x, _x,_x,_x,_x, _x,_x,_x,_x, _x,_x,_x,_x, _x,_x,_x,_x, _x,_x,_x,_x, _x,_x,_x,_x, _x,_x,_x,_x, _x,_x,_x,_x, _x,_x,_x,_x, _x,_x,_T,_T, _T,_T,_x,_x, _x,_x,_x,_x, _x,_x,_x,_x, _x,_x,_x,_x, _x,_x,_x,_x, _x,_x,_x,_x, _x,_x,_x,_x, _x,_x,_x,_x, _x,_x,_x,_x, _x,_x,_x,_x, _x,_x,_x,_x, _x,_x,_x,_x, _x,_x,_x,_x, _x,_x,_x,_x},
+		{_x,_x,_x,_x, _x,_x,_x,_x, _x,_x,_x,_x, _x,_x,_x,_x, _x,_x,_x,_x, _x,_x,_x,_x, _x,_x,_x,_x, _x,_x,_x,_x, _x,_x,_x,_x, _x,_x,_x,_T, _x,_x,_x,_x, _x,_x,_x,_T, _x,_T,_x,_x, _x,_x,_x,_x, _x,_x,_x,_x, _x,_x,_x,_x, _x,_x,_x,_x, _x,_x,_x,_x, _x,_x,_x,_x, _x,_x,_x,_x, _x,_x,_x,_x, _x,_x,_x,_x, _x,_x,_x,_x, _x,_x,_x,_x, _x,_x,_T,_T, _x,_x,_x,_x, _x,_x,_x,_x, _x,_x,_x,_x, _x,_x,_x,_x, _x,_x,_x,_x, _x,_x,_x,_x, _x,_x,_x,_x, _x,_x,_x,_x, _x,_x,_x,_x, _x,_x,_x,_x, _x,_x,_x,_x, _x,_x,_x,_x, _x,_x,_x,_x},
+		{_x,_T,_T,_x, _x,_T,_T,_T, _T,_T,_T,_T, _T,_T,_T,_T, _T,_T,_T,_T, _x,_x,_x,_x, _x,_x,_x,_x, _x,_x,_x,_x, _x,_x,_x,_x, _x,_x,_x,_x, _x,_x,_x,_x, _x,_x,_x,_x, _x,_x,_x,_x, _x,_x,_T,_x, _x,_x,_x,_x, _x,_x,_x,_x, _x,_x,_x,_T, _x,_x,_x,_x, _x,_x,_x,_x, _x,_x,_x,_x, _x,_x,_x,_x, _x,_x,_x,_x, _x,_x,_x,_x, _x,_x,_x,_x, _x,_x,_x,_x, _x,_x,_x,_x, _x,_x,_x,_x, _x,_x,_x,_x, _x,_x,_x,_x, _x,_x,_x,_x, _x,_x,_x,_x, _x,_x,_x,_x, _x,_x,_x,_x, _x,_x,_x,_x, _x,_x,_x,_x, _x,_x,_x,_x, _x,_x,_x,_x, _x,_x,_x,_x},
+		{_T,_x,_x,_x, _x,_x,_x,_x, _x,_x,_x,_x, _x,_x,_x,_x, _x,_x,_x,_x, _x,_x,_x,_x, _x,_x,_x,_x, _x,_x,_x,_x, _x,_x,_x,_x, _x,_x,_x,_T, _x,_x,_x,_x, _x,_x,_x,_T, _T,_T,_x,_x, _x,_x,_x,_x, _x,_x,_x,_x, _x,_x,_x,_x, _x,_x,_x,_x, _x,_x,_x,_x, _x,_x,_x,_x, _x,_x,_x,_x, _x,_x,_x,_x, _x,_x,_x,_x, _x,_x,_x,_x, _x,_x,_x,_x, _x,_x,_T,_T, _T,_x,_x,_x, _x,_x,_x,_x, _x,_x,_x,_x, _x,_x,_x,_x, _x,_x,_x,_x, _x,_x,_x,_x, _x,_x,_x,_x, _x,_x,_x,_x, _x,_x,_x,_x, _x,_x,_x,_x, _x,_x,_x,_x, _x,_x,_x,_x, _x,_x,_x,_x},
+		{_x,_x,_x,_x, _x,_x,_x,_x, _x,_x,_x,_x, _x,_x,_x,_x, _x,_x,_x,_x, _x,_x,_x,_x, _x,_x,_x,_x, _x,_x,_x,_x, _x,_x,_x,_x, _x,_x,_x,_x, _x,_x,_x,_x, _x,_x,_x,_x, _x,_T,_x,_x, _x,_x,_x,_x, _x,_x,_x,_x, _x,_x,_x,_x, _x,_x,_x,_x, _x,_x,_x,_x, _x,_x,_x,_x, _x,_x,_x,_x, _x,_x,_x,_x, _x,_x,_x,_x, _x,_x,_x,_x, _x,_x,_x,_x, _x,_x,_T,_T, _T,_x,_x,_x, _x,_x,_x,_x, _x,_x,_x,_x, _x,_x,_x,_x, _x,_x,_x,_x, _x,_x,_x,_x, _x,_x,_x,_x, _x,_x,_x,_x, _x,_x,_x,_x, _x,_x,_x,_x, _x,_x,_x,_x, _x,_x,_x,_x, _x,_x,_x,_x},
+		{_x,_T,_T,_T, _T,_x,_x,_x, _x,_T,_x,_T, _x,_x,_x,_x, _x,_x,_x,_x, _T,_T,_x,_x, _T,_x,_x,_x, _x,_x,_x,_x, _x,_T,_T,_x, _x,_x,_x,_x, _x,_x,_x,_x, _x,_x,_x,_x, _x,_x,_T,_x, _x,_x,_T,_x, _x,_x,_x,_x, _x,_x,_x,_T, _T,_x,_x,_T, _x,_x,_x,_x, _x,_x,_x,_x, _x,_x,_x,_x, _x,_x,_x,_x, _T,_x,_x,_x, _x,_x,_x,_x, _x,_x,_x,_x, _x,_x,_x,_x, _T,_T,_T,_x, _T,_T,_T,_T, _T,_x,_T,_T, _T,_T,_x,_x, _x,_x,_x,_x, _x,_x,_x,_x, _x,_x,_x,_x, _x,_x,_x,_x, _x,_x,_x,_x, _x,_x,_x,_x, _x,_T,_T,_T, _T,_T,_T,_T, _T,_x,_x,_x},
+		{_T,_x,_x,_x, _x,_x,_x,_x, _x,_x,_x,_x, _x,_x,_x,_x, _x,_x,_x,_x, _x,_x,_x,_x, _x,_x,_x,_x, _x,_x,_x,_x, _x,_x,_x,_x, _x,_x,_x,_T, _x,_x,_x,_x, _x,_x,_x,_T, _x,_T,_x,_x, _x,_x,_x,_x, _x,_x,_x,_x, _x,_x,_x,_x, _x,_x,_x,_x, _x,_x,_x,_x, _x,_x,_x,_x, _x,_x,_x,_x, _x,_x,_x,_x, _x,_x,_x,_x, _x,_x,_x,_x, _x,_x,_x,_x, _x,_x,_T,_T, _x,_x,_x,_x, _x,_x,_x,_x, _x,_x,_x,_x, _x,_x,_x,_x, _x,_x,_x,_x, _x,_x,_x,_x, _x,_x,_x,_x, _x,_x,_x,_x, _x,_x,_x,_x, _x,_x,_x,_x, _x,_x,_x,_x, _x,_x,_x,_x, _x,_x,_x,_x},
+		{_T,_x,_x,_x, _x,_x,_x,_x, _x,_x,_x,_x, _x,_x,_x,_x, _x,_x,_x,_x, _x,_x,_x,_x, _x,_x,_x,_x, _x,_x,_x,_x, _x,_x,_x,_x, _x,_x,_x,_T, _x,_x,_x,_x, _x,_x,_x,_x, _T,_T,_x,_x, _x,_x,_x,_x, _x,_x,_x,_x, _x,_x,_x,_x, _x,_x,_x,_x, _x,_x,_x,_x, _x,_x,_x,_x, _x,_x,_x,_x, _x,_x,_x,_x, _x,_x,_x,_x, _x,_x,_x,_x, _x,_x,_x,_x, _x,_x,_x,_T, _x,_x,_x,_x, _x,_x,_x,_x, _x,_x,_x,_x, _x,_x,_x,_x, _x,_x,_x,_x, _x,_x,_x,_x, _x,_x,_x,_x, _x,_x,_x,_x, _x,_x,_x,_x, _x,_x,_x,_x, _x,_x,_x,_x, _x,_x,_x,_x, _x,_x,_x,_x},
+		{_x,_T,_T,_T, _T,_x,_x,_x, _x,_T,_x,_T, _x,_x,_T,_T, _T,_x,_T,_T, _T,_T,_x,_x, _T,_x,_x,_x, _x,_T,_x,_x, _x,_T,_T,_x, _x,_x,_x,_x, _x,_x,_x,_x, _x,_x,_x,_x, _x,_x,_T,_x, _T,_x,_T,_x, _x,_x,_x,_x, _x,_x,_x,_x, _T,_x,_x,_T, _x,_x,_x,_x, _x,_x,_x,_x, _x,_x,_x,_x, _x,_x,_x,_x, _T,_x,_x,_x, _x,_x,_x,_x, _x,_x,_x,_x, _x,_x,_x,_x, _x,_T,_x,_x, _x,_T,_x,_T, _T,_x,_x,_T, _x,_x,_x,_x, _x,_x,_x,_x, _x,_x,_x,_x, _x,_T,_T,_T, _T,_T,_T,_T, _T,_T,_x,_x, _T,_x,_x,_x, _x,_T,_T,_T, _T,_T,_T,_T, _T,_x,_x,_x},
+		{_T,_T,_T,_T, _T,_x,_x,_x, _x,_T,_x,_T, _x,_x,_x,_x, _x,_x,_x,_x, _T,_T,_x,_x, _T,_x,_x,_x, _x,_x,_x,_x, _x,_T,_T,_x, _x,_x,_x,_x, _x,_x,_x,_x, _x,_x,_x,_x, _x,_x,_T,_x, _x,_x,_T,_x, _x,_x,_x,_x, _x,_x,_x,_T, _T,_x,_x,_T, _x,_x,_x,_x, _x,_x,_x,_x, _x,_x,_x,_x, _x,_x,_x,_x, _T,_x,_x,_x, _x,_x,_x,_x, _x,_x,_x,_x, _x,_x,_x,_x, _T,_T,_T,_x, _T,_T,_T,_T, _T,_x,_T,_T, _T,_T,_x,_x, _x,_x,_x,_x, _x,_x,_x,_x, _x,_x,_x,_x, _x,_x,_x,_x, _x,_x,_x,_x, _x,_x,_x,_x, _x,_T,_T,_T, _T,_T,_T,_T, _T,_x,_x,_x},
+		{_x,_T,_T,_T, _T,_x,_x,_x, _x,_T,_x,_T, _x,_x,_T,_T, _T,_x,_T,_T, _T,_T,_x,_x, _T,_x,_x,_x, _x,_x,_x,_x, _x,_T,_T,_x, _x,_x,_x,_x, _x,_x,_x,_x, _x,_x,_x,_x, _x,_x,_T,_x, _T,_x,_T,_x, _x,_x,_x,_x, _x,_T,_x,_T, _T,_x,_x,_T, _x,_x,_x,_x, _x,_x,_x,_x, _x,_x,_x,_x, _x,_x,_x,_x, _T,_x,_x,_x, _x,_x,_x,_x, _x,_x,_x,_x, _x,_x,_x,_x, _x,_T,_x,_x, _x,_T,_x,_T, _T,_x,_x,_T, _x,_x,_x,_x, _x,_x,_x,_x, _x,_x,_x,_x, _x,_T,_T,_T, _T,_T,_T,_T, _T,_T,_x,_x, _T,_x,_x,_x, _x,_T,_T,_T, _T,_T,_T,_T, _T,_x,_x,_x},
+		{_x,_T,_T,_T, _T,_x,_x,_x, _x,_T,_x,_T, _x,_x,_T,_T, _T,_x,_T,_T, _T,_T,_x,_x, _T,_x,_x,_x, _x,_x,_x,_x, _x,_T,_T,_x, _x,_x,_x,_x, _x,_x,_x,_x, _x,_x,_x,_x, _x,_x,_T,_x, _T,_x,_T,_x, _x,_x,_x,_x, _x,_T,_x,_x, _T,_x,_x,_T, _x,_x,_x,_x, _x,_x,_x,_x, _x,_x,_x,_x, _x,_x,_x,_x, _T,_x,_x,_x, _x,_x,_x,_x, _x,_x,_x,_x, _x,_x,_x,_x, _x,_T,_x,_x, _x,_T,_x,_T, _T,_x,_x,_T, _x,_x,_x,_x, _x,_x,_x,_x, _x,_x,_x,_x, _x,_T,_T,_T, _T,_T,_T,_T, _T,_T,_x,_x, _T,_x,_x,_x, _x,_T,_T,_T, _T,_T,_T,_T, _T,_x,_x,_x},
+		{_x,_x,_x,_x, _x,_x,_x,_x, _x,_x,_x,_x, _x,_x,_x,_x, _x,_x,_x,_x, _x,_x,_x,_x, _x,_x,_x,_x, _x,_x,_x,_x, _x,_x,_x,_x, _x,_x,_x,_T, _T,_x,_x,_x, _x,_x,_x,_T, _x,_x,_x,_x, _x,_x,_x,_x, _x,_x,_x,_x, _x,_x,_x,_x, _x,_x,_x,_x, _x,_x,_x,_x, _x,_x,_x,_x, _x,_x,_x,_x, _x,_x,_x,_x, _x,_x,_x,_x, _x,_x,_x,_x, _x,_x,_x,_x, _x,_x,_T,_x, _x,_x,_x,_x, _x,_x,_x,_x, _x,_x,_x,_x, _x,_x,_x,_x, _x,_x,_x,_x, _x,_x,_x,_x, _x,_x,_x,_x, _x,_x,_x,_x, _x,_x,_x,_x, _x,_x,_x,_x, _x,_x,_x,_x, _x,_x,_x,_x, _x,_x,_x,_x},
+		{_x,_T,_T,_T, _T,_x,_x,_x, _x,_T,_x,_T, _x,_x,_x,_x, _x,_x,_x,_x, _T,_T,_x,_x, _T,_x,_x,_x, _x,_x,_x,_x, _x,_T,_T,_T, _x,_x,_x,_x, _x,_x,_x,_x, _x,_x,_x,_x, _x,_x,_T,_T, _x,_x,_T,_x, _x,_x,_x,_x, _x,_x,_x,_T, _T,_x,_x,_T, _x,_x,_x,_x, _x,_x,_x,_x, _x,_x,_x,_x, _x,_x,_x,_x, _T,_x,_x,_x, _x,_x,_x,_x, _x,_x,_x,_x, _x,_x,_x,_x, _T,_T,_T,_x, _T,_T,_T,_T, _T,_x,_T,_T, _T,_T,_x,_x, _x,_x,_x,_x, _x,_x,_x,_x, _x,_x,_x,_x, _x,_x,_x,_x, _x,_x,_x,_x, _x,_x,_x,_x, _x,_T,_T,_T, _T,_T,_T,_T, _T,_x,_x,_x},
+		{_x,_T,_T,_T, _T,_x,_x,_x, _x,_T,_x,_T, _x,_x,_x,_x, _x,_x,_x,_x, _T,_T,_x,_x, _T,_x,_x,_x, _x,_x,_x,_x, _x,_T,_T,_T, _x,_x,_x,_x, _x,_x,_x,_x, _x,_x,_x,_x, _x,_x,_T,_T, _x,_x,_T,_x, _x,_x,_x,_x, _x,_x,_x,_T, _T,_x,_x,_T, _x,_x,_x,_x, _x,_x,_x,_x, _x,_x,_x,_x, _x,_x,_x,_x, _T,_x,_x,_x, _x,_x,_x,_x, _x,_x,_x,_x, _x,_x,_T,_T, _T,_T,_T,_x, _T,_T,_T,_T, _T,_x,_T,_T, _T,_T,_x,_x, _x,_x,_x,_x, _x,_x,_x,_x, _x,_x,_x,_x, _x,_x,_x,_x, _x,_x,_x,_x, _x,_x,_x,_x, _x,_T,_T,_T, _T,_T,_T,_T, _T,_x,_x,_x},
+		{_x,_x,_x,_x, _x,_x,_x,_x, _x,_x,_x,_x, _x,_x,_x,_x, _x,_x,_x,_x, _x,_x,_x,_x, _x,_x,_x,_x, _x,_x,_x,_x, _x,_x,_x,_x, _x,_x,_x,_x, _x,_x,_x,_x, _x,_x,_x,_x, _x,_x,_x,_x, _x,_x,_x,_x, _T,_T,_T,_T, _T,_x,_x,_x, _x,_x,_x,_x, _x,_x,_x,_x, _x,_x,_x,_x, _x,_x,_x,_x, _x,_x,_x,_x, _x,_x,_x,_x, _x,_x,_x,_x, _x,_x,_x,_x, _x,_x,_x,_x, _x,_x,_x,_x, _x,_x,_x,_x, _x,_x,_x,_x, _x,_x,_x,_T, _T,_T,_T,_T, _T,_T,_T,_T, _T,_x,_x,_x, _x,_x,_x,_x, _x,_x,_x,_x, _x,_x,_x,_x, _x,_x,_x,_x, _x,_x,_x,_x, _x,_x,_x,_x},
+		{_x,_T,_T,_T, _T,_x,_x,_x, _x,_T,_x,_T, _x,_x,_T,_T, _T,_x,_T,_T, _T,_T,_x,_x, _T,_x,_x,_x, _x,_x,_x,_x, _x,_T,_T,_x, _x,_x,_x,_x, _x,_x,_x,_x, _x,_x,_x,_x, _x,_x,_T,_x, _T,_x,_T,_x, _x,_x,_x,_x, _x,_T,_x,_x, _T,_x,_x,_T, _x,_x,_x,_x, _x,_x,_x,_x, _x,_x,_x,_x, _x,_x,_x,_x, _T,_x,_x,_x, _x,_x,_T,_x, _x,_x,_x,_x, _x,_x,_x,_x, _x,_T,_x,_x, _x,_T,_x,_T, _T,_x,_x,_T, _x,_x,_x,_x, _x,_x,_x,_x, _x,_x,_x,_x, _x,_T,_T,_T, _T,_T,_T,_T, _T,_T,_x,_x, _T,_x,_x,_x, _x,_T,_T,_T, _T,_T,_T,_T, _T,_x,_x,_x},
+		{_x,_x,_T,_T, _T,_x,_x,_x, _x,_T,_x,_T, _x,_x,_x,_x, _x,_x,_x,_x, _T,_T,_x,_x, _T,_x,_x,_x, _x,_x,_x,_x, _x,_x,_x,_x, _x,_x,_x,_x, _x,_x,_x,_x, _x,_x,_x,_x, _x,_x,_x,_x, _x,_x,_T,_x, _x,_x,_x,_x, _x,_x,_x,_x, _x,_x,_x,_x, _x,_x,_x,_x, _x,_x,_x,_x, _x,_x,_x,_x, _x,_x,_x,_x, _x,_x,_x,_x, _x,_x,_x,_x, _x,_x,_x,_x, _x,_x,_x,_x, _x,_x,_x,_x, _x,_x,_x,_x, _x,_x,_x,_x, _x,_x,_x,_x, _x,_x,_x,_x, _x,_x,_x,_x, _x,_x,_x,_x, _x,_x,_x,_x, _x,_x,_x,_x, _x,_x,_x,_x, _x,_T,_T,_T, _T,_T,_T,_T, _T,_x,_x,_x},
+		{_T,_T,_T,_T, _T,_x,_x,_x, _x,_T,_x,_T, _x,_x,_x,_x, _x,_x,_x,_x, _T,_T,_x,_x, _T,_x,_x,_x, _x,_x,_x,_x, _x,_T,_T,_T, _x,_x,_x,_x, _x,_x,_x,_x, _x,_x,_x,_x, _x,_x,_T,_T, _x,_x,_T,_x, _x,_x,_x,_x, _x,_x,_x,_T, _T,_x,_x,_T, _x,_x,_x,_x, _x,_x,_x,_x, _x,_x,_x,_x, _x,_x,_x,_x, _T,_x,_x,_x, _x,_x,_x,_x, _x,_x,_x,_x, _x,_x,_x,_x, _T,_T,_T,_x, _T,_T,_T,_T, _T,_x,_T,_T, _T,_T,_x,_x, _x,_x,_x,_x, _x,_x,_x,_x, _x,_x,_x,_x, _x,_x,_x,_x, _x,_x,_x,_x, _x,_x,_x,_x, _x,_T,_T,_T, _T,_T,_T,_T, _T,_x,_x,_x},
+		{_x,_T,_T,_T, _T,_x,_x,_x, _x,_T,_x,_T, _x,_x,_T,_T, _T,_x,_T,_T, _T,_T,_x,_x, _T,_x,_x,_x, _x,_x,_x,_x, _x,_T,_T,_x, _x,_x,_x,_x, _x,_x,_x,_x, _x,_x,_x,_x, _x,_x,_T,_x, _T,_x,_T,_x, _x,_x,_x,_x, _x,_x,_x,_x, _T,_x,_x,_T, _x,_x,_x,_x, _x,_x,_x,_x, _x,_x,_x,_x, _x,_x,_x,_x, _T,_x,_x,_x, _x,_x,_x,_x, _x,_x,_x,_x, _x,_x,_x,_x, _x,_T,_x,_x, _x,_T,_x,_T, _T,_x,_x,_T, _x,_x,_x,_x, _x,_x,_x,_x, _x,_x,_x,_x, _x,_x,_x,_x, _x,_T,_T,_T, _T,_T,_x,_x, _T,_x,_x,_x, _x,_T,_T,_T, _T,_T,_T,_T, _T,_x,_x,_x},
+		{_x,_x,_x,_x, _x,_x,_x,_x, _x,_x,_x,_x, _x,_x,_T,_T, _x,_x,_T,_T, _x,_x,_x,_x, _x,_x,_x,_x, _x,_x,_x,_x, _x,_T,_T,_x, _x,_x,_x,_x, _x,_x,_x,_x, _x,_x,_x,_x, _x,_x,_x,_x, _x,_x,_x,_x, _x,_x,_x,_x, _x,_x,_x,_x, _T,_x,_x,_T, _x,_x,_x,_x, _x,_x,_x,_x, _x,_x,_x,_x, _x,_x,_x,_x, _T,_x,_x,_x, _x,_x,_x,_x, _x,_x,_x,_x, _x,_x,_x,_x, _x,_T,_x,_x, _x,_T,_x,_T, _T,_x,_x,_T, _x,_x,_x,_x, _x,_x,_x,_x, _x,_x,_x,_x, _x,_x,_x,_x, _x,_x,_x,_T, _T,_T,_x,_x, _x,_x,_x,_x, _x,_x,_x,_x, _x,_x,_x,_x, _x,_x,_x,_x},
+		{_T,_T,_T,_T, _T,_x,_x,_x, _x,_T,_x,_T, _x,_x,_x,_x, _x,_x,_x,_x, _T,_T,_T,_T, _T,_T,_T,_T, _T,_T,_T,_T, _T,_T,_T,_T, _T,_T,_T,_T, _T,_T,_T,_T, _T,_T,_T,_T, _T,_T,_T,_T, _T,_T,_T,_T, _T,_T,_T,_T, _T,_T,_T,_T, _T,_x,_T,_T, _T,_T,_T,_T, _x,_T,_x,_x, _T,_x,_x,_x, _T,_T,_T,_T, _T,_T,_T,_T, _T,_T,_x,_T, _x,_x,_T,_T, _T,_T,_T,_T, _T,_T,_T,_x, _T,_T,_T,_T, _T,_T,_T,_T, _T,_T,_x,_T, _T,_T,_T,_T, _T,_T,_T,_T, _T,_T,_T,_T, _T,_T,_x,_x, _x,_x,_T,_T, _T,_T,_T,_T, _T,_T,_T,_T, _T,_T,_T,_T, _T,_T,_x,_x},
+		{_T,_T,_T,_T, _T,_x,_x,_x, _x,_T,_x,_T, _x,_x,_x,_x, _x,_x,_x,_x, _T,_T,_T,_T, _T,_T,_x,_T, _x,_T,_T,_T, _T,_T,_T,_T, _T,_T,_T,_T, _T,_T,_T,_T, _T,_T,_T,_T, _T,_T,_T,_T, _x,_T,_T,_T, _T,_T,_T,_T, _T,_T,_T,_T, _T,_x,_T,_T, _T,_T,_T,_T, _x,_T,_x,_x, _T,_x,_x,_x, _T,_T,_T,_T, _T,_T,_T,_T, _T,_T,_x,_T, _x,_x,_T,_T, _T,_T,_T,_T, _T,_T,_T,_x, _T,_T,_T,_T, _T,_T,_T,_T, _T,_T,_x,_T, _T,_T,_T,_T, _T,_T,_T,_T, _T,_T,_T,_T, _T,_T,_x,_x, _x,_x,_T,_T, _T,_T,_T,_T, _T,_T,_T,_T, _T,_T,_T,_T, _T,_T,_x,_x}
 
   };
 } // end Parser
@@ -5255,193 +5265,194 @@ public class Errors {
 			case 85: s = "\"const\" expected"; break;
 			case 86: s = "\":=\" expected"; break;
 			case 87: s = "\"newtype\" expected"; break;
-			case 88: s = "\"type\" expected"; break;
-			case 89: s = "\"new\" expected"; break;
-			case 90: s = "\"iterator\" expected"; break;
-			case 91: s = "\"yields\" expected"; break;
-			case 92: s = "\"returns\" expected"; break;
-			case 93: s = "\"method\" expected"; break;
-			case 94: s = "\"colemma\" expected"; break;
-			case 95: s = "\"comethod\" expected"; break;
-			case 96: s = "\"constructor\" expected"; break;
-			case 97: s = "\"free\" expected"; break;
-			case 98: s = "\"ensures\" expected"; break;
-			case 99: s = "\"yield\" expected"; break;
-			case 100: s = "\"label\" expected"; break;
-			case 101: s = "\"break\" expected"; break;
-			case 102: s = "\"where\" expected"; break;
-			case 103: s = "\"return\" expected"; break;
-			case 104: s = "\"if\" expected"; break;
-			case 105: s = "\"while\" expected"; break;
-			case 106: s = "\"match\" expected"; break;
-			case 107: s = "\"assert\" expected"; break;
-			case 108: s = "\"by\" expected"; break;
-			case 109: s = "\"print\" expected"; break;
-			case 110: s = "\"forall\" expected"; break;
-			case 111: s = "\"parallel\" expected"; break;
-			case 112: s = "\"modify\" expected"; break;
-			case 113: s = "\"#\" expected"; break;
-			case 114: s = "\"<=\" expected"; break;
-			case 115: s = "\">=\" expected"; break;
-			case 116: s = "\"\\u2264\" expected"; break;
-			case 117: s = "\"\\u2265\" expected"; break;
-			case 118: s = "\"<==>\" expected"; break;
-			case 119: s = "\"\\u21d4\" expected"; break;
-			case 120: s = "\"==>\" expected"; break;
-			case 121: s = "\"\\u21d2\" expected"; break;
-			case 122: s = "\"<==\" expected"; break;
-			case 123: s = "\"\\u21d0\" expected"; break;
-			case 124: s = "\"&&\" expected"; break;
-			case 125: s = "\"\\u2227\" expected"; break;
-			case 126: s = "\"||\" expected"; break;
-			case 127: s = "\"\\u2228\" expected"; break;
-			case 128: s = "\"!\" expected"; break;
-			case 129: s = "\"\\u00ac\" expected"; break;
-			case 130: s = "\"\\u2200\" expected"; break;
-			case 131: s = "\"exists\" expected"; break;
-			case 132: s = "\"\\u2203\" expected"; break;
-			case 133: s = "\"in\" expected"; break;
-			case 134: s = "\"+\" expected"; break;
-			case 135: s = "\"-\" expected"; break;
-			case 136: s = "\"/\" expected"; break;
-			case 137: s = "\"%\" expected"; break;
-			case 138: s = "\"&\" expected"; break;
-			case 139: s = "\"^\" expected"; break;
-			case 140: s = "\"false\" expected"; break;
-			case 141: s = "\"true\" expected"; break;
-			case 142: s = "\"null\" expected"; break;
-			case 143: s = "\"this\" expected"; break;
-			case 144: s = "\"fresh\" expected"; break;
-			case 145: s = "\"allocated\" expected"; break;
-			case 146: s = "\"unchanged\" expected"; break;
-			case 147: s = "\"old\" expected"; break;
-			case 148: s = "\"..\" expected"; break;
-			case 149: s = "??? expected"; break;
-			case 150: s = "invalid TopDecl"; break;
-			case 151: s = "invalid DeclModifier"; break;
-			case 152: s = "invalid SubModuleDecl"; break;
-			case 153: s = "this symbol not expected in SubModuleDecl"; break;
-			case 154: s = "invalid SubModuleDecl"; break;
+			case 88: s = "\"witness\" expected"; break;
+			case 89: s = "\"type\" expected"; break;
+			case 90: s = "\"new\" expected"; break;
+			case 91: s = "\"iterator\" expected"; break;
+			case 92: s = "\"yields\" expected"; break;
+			case 93: s = "\"returns\" expected"; break;
+			case 94: s = "\"method\" expected"; break;
+			case 95: s = "\"colemma\" expected"; break;
+			case 96: s = "\"comethod\" expected"; break;
+			case 97: s = "\"constructor\" expected"; break;
+			case 98: s = "\"free\" expected"; break;
+			case 99: s = "\"ensures\" expected"; break;
+			case 100: s = "\"yield\" expected"; break;
+			case 101: s = "\"label\" expected"; break;
+			case 102: s = "\"break\" expected"; break;
+			case 103: s = "\"where\" expected"; break;
+			case 104: s = "\"return\" expected"; break;
+			case 105: s = "\"if\" expected"; break;
+			case 106: s = "\"while\" expected"; break;
+			case 107: s = "\"match\" expected"; break;
+			case 108: s = "\"assert\" expected"; break;
+			case 109: s = "\"by\" expected"; break;
+			case 110: s = "\"print\" expected"; break;
+			case 111: s = "\"forall\" expected"; break;
+			case 112: s = "\"parallel\" expected"; break;
+			case 113: s = "\"modify\" expected"; break;
+			case 114: s = "\"#\" expected"; break;
+			case 115: s = "\"<=\" expected"; break;
+			case 116: s = "\">=\" expected"; break;
+			case 117: s = "\"\\u2264\" expected"; break;
+			case 118: s = "\"\\u2265\" expected"; break;
+			case 119: s = "\"<==>\" expected"; break;
+			case 120: s = "\"\\u21d4\" expected"; break;
+			case 121: s = "\"==>\" expected"; break;
+			case 122: s = "\"\\u21d2\" expected"; break;
+			case 123: s = "\"<==\" expected"; break;
+			case 124: s = "\"\\u21d0\" expected"; break;
+			case 125: s = "\"&&\" expected"; break;
+			case 126: s = "\"\\u2227\" expected"; break;
+			case 127: s = "\"||\" expected"; break;
+			case 128: s = "\"\\u2228\" expected"; break;
+			case 129: s = "\"!\" expected"; break;
+			case 130: s = "\"\\u00ac\" expected"; break;
+			case 131: s = "\"\\u2200\" expected"; break;
+			case 132: s = "\"exists\" expected"; break;
+			case 133: s = "\"\\u2203\" expected"; break;
+			case 134: s = "\"in\" expected"; break;
+			case 135: s = "\"+\" expected"; break;
+			case 136: s = "\"-\" expected"; break;
+			case 137: s = "\"/\" expected"; break;
+			case 138: s = "\"%\" expected"; break;
+			case 139: s = "\"&\" expected"; break;
+			case 140: s = "\"^\" expected"; break;
+			case 141: s = "\"false\" expected"; break;
+			case 142: s = "\"true\" expected"; break;
+			case 143: s = "\"null\" expected"; break;
+			case 144: s = "\"this\" expected"; break;
+			case 145: s = "\"fresh\" expected"; break;
+			case 146: s = "\"allocated\" expected"; break;
+			case 147: s = "\"unchanged\" expected"; break;
+			case 148: s = "\"old\" expected"; break;
+			case 149: s = "\"..\" expected"; break;
+			case 150: s = "??? expected"; break;
+			case 151: s = "invalid TopDecl"; break;
+			case 152: s = "invalid DeclModifier"; break;
+			case 153: s = "invalid SubModuleDecl"; break;
+			case 154: s = "this symbol not expected in SubModuleDecl"; break;
 			case 155: s = "invalid SubModuleDecl"; break;
 			case 156: s = "invalid SubModuleDecl"; break;
-			case 157: s = "this symbol not expected in ClassDecl"; break;
-			case 158: s = "this symbol not expected in DatatypeDecl"; break;
-			case 159: s = "invalid DatatypeDecl"; break;
-			case 160: s = "this symbol not expected in DatatypeDecl"; break;
-			case 161: s = "invalid NewtypeDecl"; break;
-			case 162: s = "invalid OtherTypeDecl"; break;
-			case 163: s = "this symbol not expected in OtherTypeDecl"; break;
-			case 164: s = "this symbol not expected in IteratorDecl"; break;
-			case 165: s = "invalid IteratorDecl"; break;
-			case 166: s = "this symbol not expected in TraitDecl"; break;
-			case 167: s = "invalid ClassMemberDecl"; break;
-			case 168: s = "invalid QualifiedModuleExportSuffix"; break;
+			case 157: s = "invalid SubModuleDecl"; break;
+			case 158: s = "this symbol not expected in ClassDecl"; break;
+			case 159: s = "this symbol not expected in DatatypeDecl"; break;
+			case 160: s = "invalid DatatypeDecl"; break;
+			case 161: s = "this symbol not expected in DatatypeDecl"; break;
+			case 162: s = "invalid NewtypeDecl"; break;
+			case 163: s = "invalid OtherTypeDecl"; break;
+			case 164: s = "this symbol not expected in OtherTypeDecl"; break;
+			case 165: s = "this symbol not expected in IteratorDecl"; break;
+			case 166: s = "invalid IteratorDecl"; break;
+			case 167: s = "this symbol not expected in TraitDecl"; break;
+			case 168: s = "invalid ClassMemberDecl"; break;
 			case 169: s = "invalid QualifiedModuleExportSuffix"; break;
-			case 170: s = "invalid DotSuffix"; break;
-			case 171: s = "this symbol not expected in FieldDecl"; break;
-			case 172: s = "this symbol not expected in ConstantFieldDecl"; break;
-			case 173: s = "invalid FunctionDecl"; break;
+			case 170: s = "invalid QualifiedModuleExportSuffix"; break;
+			case 171: s = "invalid DotSuffix"; break;
+			case 172: s = "this symbol not expected in FieldDecl"; break;
+			case 173: s = "this symbol not expected in ConstantFieldDecl"; break;
 			case 174: s = "invalid FunctionDecl"; break;
 			case 175: s = "invalid FunctionDecl"; break;
 			case 176: s = "invalid FunctionDecl"; break;
 			case 177: s = "invalid FunctionDecl"; break;
 			case 178: s = "invalid FunctionDecl"; break;
-			case 179: s = "this symbol not expected in MethodDecl"; break;
-			case 180: s = "invalid MethodDecl"; break;
+			case 179: s = "invalid FunctionDecl"; break;
+			case 180: s = "this symbol not expected in MethodDecl"; break;
 			case 181: s = "invalid MethodDecl"; break;
-			case 182: s = "invalid FIdentType"; break;
-			case 183: s = "this symbol not expected in OldSemi"; break;
-			case 184: s = "invalid TypeIdentOptional"; break;
-			case 185: s = "invalid TypeAndToken"; break;
-			case 186: s = "this symbol not expected in IteratorSpec"; break;
-			case 187: s = "invalid IteratorSpec"; break;
+			case 182: s = "invalid MethodDecl"; break;
+			case 183: s = "invalid FIdentType"; break;
+			case 184: s = "this symbol not expected in OldSemi"; break;
+			case 185: s = "invalid TypeIdentOptional"; break;
+			case 186: s = "invalid TypeAndToken"; break;
+			case 187: s = "this symbol not expected in IteratorSpec"; break;
 			case 188: s = "invalid IteratorSpec"; break;
-			case 189: s = "this symbol not expected in MethodSpec"; break;
-			case 190: s = "invalid MethodSpec"; break;
+			case 189: s = "invalid IteratorSpec"; break;
+			case 190: s = "this symbol not expected in MethodSpec"; break;
 			case 191: s = "invalid MethodSpec"; break;
-			case 192: s = "invalid FrameExpression"; break;
-			case 193: s = "this symbol not expected in FunctionSpec"; break;
-			case 194: s = "invalid FunctionSpec"; break;
-			case 195: s = "invalid PossiblyWildFrameExpression"; break;
-			case 196: s = "invalid PossiblyWildExpression"; break;
-			case 197: s = "this symbol not expected in OneStmt"; break;
-			case 198: s = "invalid OneStmt"; break;
-			case 199: s = "this symbol not expected in OneStmt"; break;
-			case 200: s = "invalid OneStmt"; break;
-			case 201: s = "invalid AssertStmt"; break;
+			case 192: s = "invalid MethodSpec"; break;
+			case 193: s = "invalid FrameExpression"; break;
+			case 194: s = "this symbol not expected in FunctionSpec"; break;
+			case 195: s = "invalid FunctionSpec"; break;
+			case 196: s = "invalid PossiblyWildFrameExpression"; break;
+			case 197: s = "invalid PossiblyWildExpression"; break;
+			case 198: s = "this symbol not expected in OneStmt"; break;
+			case 199: s = "invalid OneStmt"; break;
+			case 200: s = "this symbol not expected in OneStmt"; break;
+			case 201: s = "invalid OneStmt"; break;
 			case 202: s = "invalid AssertStmt"; break;
-			case 203: s = "invalid AssumeStmt"; break;
-			case 204: s = "invalid UpdateStmt"; break;
+			case 203: s = "invalid AssertStmt"; break;
+			case 204: s = "invalid AssumeStmt"; break;
 			case 205: s = "invalid UpdateStmt"; break;
-			case 206: s = "this symbol not expected in VarDeclStatement"; break;
-			case 207: s = "invalid VarDeclStatement"; break;
+			case 206: s = "invalid UpdateStmt"; break;
+			case 207: s = "this symbol not expected in VarDeclStatement"; break;
 			case 208: s = "invalid VarDeclStatement"; break;
-			case 209: s = "invalid IfStmt"; break;
+			case 209: s = "invalid VarDeclStatement"; break;
 			case 210: s = "invalid IfStmt"; break;
-			case 211: s = "invalid WhileStmt"; break;
+			case 211: s = "invalid IfStmt"; break;
 			case 212: s = "invalid WhileStmt"; break;
-			case 213: s = "invalid MatchStmt"; break;
-			case 214: s = "invalid ForallStmt"; break;
+			case 213: s = "invalid WhileStmt"; break;
+			case 214: s = "invalid MatchStmt"; break;
 			case 215: s = "invalid ForallStmt"; break;
-			case 216: s = "invalid CalcStmt"; break;
-			case 217: s = "invalid ModifyStmt"; break;
-			case 218: s = "this symbol not expected in ModifyStmt"; break;
-			case 219: s = "invalid ModifyStmt"; break;
-			case 220: s = "invalid ReturnStmt"; break;
-			case 221: s = "invalid Rhs"; break;
-			case 222: s = "invalid Lhs"; break;
-			case 223: s = "invalid CasePattern"; break;
-			case 224: s = "invalid AlternativeBlock"; break;
-			case 225: s = "invalid Guard"; break;
-			case 226: s = "invalid AlternativeBlockCase"; break;
-			case 227: s = "this symbol not expected in AlternativeBlockCase"; break;
+			case 216: s = "invalid ForallStmt"; break;
+			case 217: s = "invalid CalcStmt"; break;
+			case 218: s = "invalid ModifyStmt"; break;
+			case 219: s = "this symbol not expected in ModifyStmt"; break;
+			case 220: s = "invalid ModifyStmt"; break;
+			case 221: s = "invalid ReturnStmt"; break;
+			case 222: s = "invalid Rhs"; break;
+			case 223: s = "invalid Lhs"; break;
+			case 224: s = "invalid CasePattern"; break;
+			case 225: s = "invalid AlternativeBlock"; break;
+			case 226: s = "invalid Guard"; break;
+			case 227: s = "invalid AlternativeBlockCase"; break;
 			case 228: s = "this symbol not expected in AlternativeBlockCase"; break;
-			case 229: s = "this symbol not expected in LoopSpec"; break;
+			case 229: s = "this symbol not expected in AlternativeBlockCase"; break;
 			case 230: s = "this symbol not expected in LoopSpec"; break;
 			case 231: s = "this symbol not expected in LoopSpec"; break;
-			case 232: s = "invalid LoopSpec"; break;
-			case 233: s = "invalid CaseStatement"; break;
-			case 234: s = "this symbol not expected in CaseStatement"; break;
+			case 232: s = "this symbol not expected in LoopSpec"; break;
+			case 233: s = "invalid LoopSpec"; break;
+			case 234: s = "invalid CaseStatement"; break;
 			case 235: s = "this symbol not expected in CaseStatement"; break;
-			case 236: s = "invalid CalcOp"; break;
-			case 237: s = "invalid EquivOp"; break;
-			case 238: s = "invalid ImpliesOp"; break;
-			case 239: s = "invalid ExpliesOp"; break;
-			case 240: s = "invalid AndOp"; break;
-			case 241: s = "invalid OrOp"; break;
-			case 242: s = "invalid NegOp"; break;
-			case 243: s = "invalid Forall"; break;
-			case 244: s = "invalid Exists"; break;
-			case 245: s = "invalid QSep"; break;
-			case 246: s = "invalid ImpliesExpliesExpression"; break;
-			case 247: s = "invalid LogicalExpression"; break;
+			case 236: s = "this symbol not expected in CaseStatement"; break;
+			case 237: s = "invalid CalcOp"; break;
+			case 238: s = "invalid EquivOp"; break;
+			case 239: s = "invalid ImpliesOp"; break;
+			case 240: s = "invalid ExpliesOp"; break;
+			case 241: s = "invalid AndOp"; break;
+			case 242: s = "invalid OrOp"; break;
+			case 243: s = "invalid NegOp"; break;
+			case 244: s = "invalid Forall"; break;
+			case 245: s = "invalid Exists"; break;
+			case 246: s = "invalid QSep"; break;
+			case 247: s = "invalid ImpliesExpliesExpression"; break;
 			case 248: s = "invalid LogicalExpression"; break;
-			case 249: s = "invalid ShiftTerm"; break;
-			case 250: s = "invalid RelOp"; break;
-			case 251: s = "invalid AddOp"; break;
-			case 252: s = "invalid BitvectorFactor"; break;
-			case 253: s = "invalid MulOp"; break;
-			case 254: s = "invalid UnaryExpression"; break;
-			case 255: s = "invalid Suffix"; break;
+			case 249: s = "invalid LogicalExpression"; break;
+			case 250: s = "invalid ShiftTerm"; break;
+			case 251: s = "invalid RelOp"; break;
+			case 252: s = "invalid AddOp"; break;
+			case 253: s = "invalid BitvectorFactor"; break;
+			case 254: s = "invalid MulOp"; break;
+			case 255: s = "invalid UnaryExpression"; break;
 			case 256: s = "invalid Suffix"; break;
 			case 257: s = "invalid Suffix"; break;
 			case 258: s = "invalid Suffix"; break;
 			case 259: s = "invalid Suffix"; break;
-			case 260: s = "invalid LambdaExpression"; break;
-			case 261: s = "invalid EndlessExpression"; break;
+			case 260: s = "invalid Suffix"; break;
+			case 261: s = "invalid LambdaExpression"; break;
 			case 262: s = "invalid EndlessExpression"; break;
-			case 263: s = "invalid NameSegment"; break;
-			case 264: s = "invalid DisplayExpr"; break;
-			case 265: s = "invalid MultiSetExpr"; break;
-			case 266: s = "invalid ConstAtomExpression"; break;
-			case 267: s = "invalid Nat"; break;
-			case 268: s = "invalid LambdaArrow"; break;
-			case 269: s = "invalid MatchExpression"; break;
-			case 270: s = "invalid QuantifierGuts"; break;
-			case 271: s = "invalid StmtInExpr"; break;
-			case 272: s = "invalid LetExpr"; break;
-			case 273: s = "invalid CaseExpression"; break;
-			case 274: s = "invalid MemberBindingUpdate"; break;
+			case 263: s = "invalid EndlessExpression"; break;
+			case 264: s = "invalid NameSegment"; break;
+			case 265: s = "invalid DisplayExpr"; break;
+			case 266: s = "invalid MultiSetExpr"; break;
+			case 267: s = "invalid ConstAtomExpression"; break;
+			case 268: s = "invalid Nat"; break;
+			case 269: s = "invalid LambdaArrow"; break;
+			case 270: s = "invalid MatchExpression"; break;
+			case 271: s = "invalid QuantifierGuts"; break;
+			case 272: s = "invalid StmtInExpr"; break;
+			case 273: s = "invalid LetExpr"; break;
+			case 274: s = "invalid CaseExpression"; break;
+			case 275: s = "invalid MemberBindingUpdate"; break;
 
       default: s = "error " + n; break;
     }
