Test/dafny0/NewtypesResolution.dfy
@@ -249,3 +249,33 @@ module IntegerBasedValues {
     m' := m[t := 1.1415];  // error: real is not an integer-based numeric type
   }
 }
+
+module CompilableWitnesses {
+  type XX = c: bool | true
+    witness
+      ghost var g := false; g  // error: witness must be compilable
+  newtype XX' = c: int | true
+    witness
+      ghost var g := 0; g  // error: witness must be compilable
+  type YY = c: bool | true
+    witness
+      forall x: int :: 0 <= x < 100  // error: witness must be compilable
+  newtype YY' = c: int | true
+    witness
+      if forall x: int :: 0 <= x < 100 then 1 else 3  // error: witness must be compilable
+}
+
+module Regression {
+  // The following are regression tests for what once had caused the resolver to crash
+  type CC = c: bool | forall d: DD :: true
+  type CC' = c: bool | false in set d: DD | true
+  type DD = d: bool | true
+}
+
+module CycleViaConstraintsOrWitnesses {
+  type AA = a: int | true witness var b: BB := 0; if b < 100 then 0 else 2  // error: cycle
+  type BB = b: int | var a: CC := 0; a < 1  // error: cycle
+  type CC = c: int | forall d: DD :: d == d  // error: cycle
+  newtype DD = d: int | true witness var e: EE := 0; if e < 100 then 0 else 2  // error: cycle
+  newtype EE = e: int | var a: AA := 0; a < 1  // error: cycle
+}
